Port Aesop from Lean fork
Between the last commit and this one, Aesop was developed as part of a
Lean fork because certain features were only available to the standard
library. These features are now available to user code, so we resume
development here.

Aesop/RuleBuilder.lean
@@ -1,67 +1,143 @@
 /-
 Copyright (c) 2021 Jannis Limperg. All rights reserved.
 Released under Apache 2.0 license as described in the file LICENSE.
-Authors: Jannis Limperg, Asta Halkjær From
+Authors: Jannis Limperg
 -/
 
 import Aesop.Rule
-
-namespace Aesop
+import Aesop.RuleTac
+import Lean.Meta.Tactic.Simp.SimpLemmas
 
 open Lean
 open Lean.Meta
-open Lean.Elab.Tactic (Tactic TacticM evalTactic)
-open Lean.Elab.Term (evalExpr)
 
-inductive RuleBuilderOutput (α : Type) : Type
-| rule (r : Rule α) (imode : IndexingMode)
-| simpLemmas (s : SimpLemmas)
+namespace Aesop
+
+structure RegularRuleBuilderResult where
+  builderName : Name
+  tac : RuleTac
+  indexingMode : IndexingMode
   deriving Inhabited
 
-def RuleBuilder α := DefinitionVal → TacticM (RuleBuilderOutput α)
+inductive NormRuleBuilderResult
+  | regular (r : RegularRuleBuilderResult)
+  | simpEntries (es : Array SimpEntry)
+  deriving Inhabited
+
+inductive RuleIdent
+  | const (decl : Name)
+  | fvar (userName : Name)
+  deriving Inhabited
+
+namespace RuleIdent
+
+instance : ToFormat RuleIdent where
+  format
+    | const decl => format decl
+    | fvar userName => format userName
+
+protected def type : RuleIdent → MetaM Expr
+  | const c => return (← getConstInfo c).type
+  | fvar userName => return (← getLocalDeclFromUserName userName).type
+
+protected def ruleName : RuleIdent → Name
+  | const c => `global ++ c
+  | fvar userName => `local ++ userName
+
+protected def ofName (n : Name) : MetaM RuleIdent := do
+  try
+    let _ ← getLocalDeclFromUserName n
+    pure $ fvar n
+  catch _ =>
+    pure $ const n
+
+end RuleIdent
+
+abbrev RuleBuilder α := RuleIdent → MetaM α
 
 namespace RuleBuilder
 
-unsafe def tac : RuleBuilder α := λ c =>
-  match c.type with
-  -- TODO: is this correct?
-  | `(tactic| $n) => do
-    let t ← evalExpr (MVarId → MetaM (List MVarId)) c.name c.value
-    pure $ RuleBuilderOutput.rule
-      { tac := t,
-        name := c.name,
-        priorityInfo := sorry } -- How do we come up with this?
-      IndexingMode.unindexed
-  | _ => panic! "Expected {d.to_name} to have type `tactic`."
+def normSimpUnfold : RuleBuilder NormRuleBuilderResult
+  | RuleIdent.const decl => do
+    let info ← getConstInfo decl
+    unless info.hasValue do
+      throwError "aesop: expected {decl} to be a definition to unfold"
+    return NormRuleBuilderResult.simpEntries #[SimpEntry.toUnfold decl]
+  | RuleIdent.fvar _ =>
+    throwError "aesop: local hypotheses cannot be added as simp lemmas"
 
-def applyIndexingMode (type : Expr) : TacticM IndexingMode := do
-  let headConstant ← conclusionHeadConstant? type
-  pure $
-    match headConstant with
-    | some c => indexTarget (toExpr c)
-    | none => unindexed
+def normSimpLemmas : RuleBuilder NormRuleBuilderResult
+  | RuleIdent.const decl => do
+    let info ← getConstInfo decl
+    unless (← isProp info.type) do
+      throwError "aesop: tried to add {decl} as a simp lemma, but it is not a proposition"
+    let simpLemmas ← mkSimpLemmasFromConst decl (post := true) (prio := 0)
+      -- TODO I don't really know what the `post` and `prio` above mean.
+    return NormRuleBuilderResult.simpEntries $ simpLemmas.map SimpEntry.lemma
+  | RuleIdent.fvar _ => do
+    throwError "aesop: local hypotheses cannot be added as simp lemmas"
 
-def apply : RuleBuilder α := λ c => do
-  let imode ← applyIndexingMode c.type
-  let n := c.name
-  pure $ RuleBuilderOutput.rule
-    { tac := flip Meta.apply (mkConst n),
-      name := "apply {n}",
-      priorityInfo := sorry } -- TODO
-    imode
+def applyIndexingMode (type : Expr) : MetaM IndexingMode := do
+  let savedState ← saveState
+  let path ←
+    try
+      let (_, _, conclusion) ← forallMetaTelescope type
+      DiscrTree.mkPath conclusion
+    finally
+      restoreState savedState
+  -- We use a meta telescope because `DiscrTree.mkPath` ignores metas (they
+  -- turn into `Key.star`) but not fvars.
+  return IndexingMode.indexTarget path
 
-def normalizationSimpLemma : RuleBuilder α := λ c => do
-  let n := c.name
-  let s ← SimpLemmas.empty.addConst n
-    -- TODO: unsure how this fail! stuff works now
-    -- <|> fail! "Expected {n} to be a (conditional) equation that can be used as a simp lemma."
-  pure $ RuleBuilderOutput.simpLemmas s
+def apply : RuleBuilder RegularRuleBuilderResult := λ ruleIdent => do
+  let type := (← ruleIdent.type)
+  let tac ←
+    match ruleIdent with
+    | RuleIdent.const decl => RuleTacBuilder.apply decl
+    | RuleIdent.fvar userName => RuleTacBuilder.applyFVar userName
+  return {
+    builderName := `apply
+    tac := tac
+    indexingMode := (← applyIndexingMode type)
+  }
 
-unsafe def normalizationDefault : RuleBuilder α := λ c =>
-  tac c <|> normalizationSimpLemma c
-    -- TODO: unsure how this fail! stuff works now
-    -- <|> fail! "Expected {c.to_name} to have type `tactic unit` or to be suitable as a simp lemma."
+def tactic : RuleBuilder RegularRuleBuilderResult
+  | RuleIdent.const decl =>
+    return {
+      builderName := `tactic
+      tac := (← RuleTacBuilder.tactic decl)
+      indexingMode := IndexingMode.unindexed
+    }
+  | RuleIdent.fvar _ =>
+    throwError "aesop: tactic builder does not support local hypotheses."
 
-end RuleBuilder
+-- TODO In the default builders below, we should distinguish between fatal and
+-- nonfatal errors. E.g. if the `tactic` builder finds a declaration that is not
+-- of tactic type, this is a nonfatal error and we should continue with the next
+-- builder. But if the simp builder finds an equation that cannot be interpreted
+-- as a simp lemma for some reason, this is a fatal error. Continuing with the
+-- next builder is more confusing than anything because the user probably
+-- intended to add a simp lemma.
 
-end Aesop
+def unsafeRuleDefault : RuleBuilder RegularRuleBuilderResult
+  | i@(RuleIdent.const _) => tactic i <|> apply i <|> err i
+  | i@(RuleIdent.fvar _) => apply i <|> err i
+  where
+    err i := throwError "aesop: Unable to interpret {i} as an unsafe rule."
+
+def safeRuleDefault : RuleBuilder RegularRuleBuilderResult
+  | i@(RuleIdent.const _) => tactic i <|> apply i <|> err i
+  | i@(RuleIdent.fvar _) => apply i <|> err i
+  where
+    err i := throwError "aesop: Unable to interpret {i} as a safe rule."
+
+def normRuleDefault : RuleBuilder NormRuleBuilderResult
+  | i@(RuleIdent.const _) =>
+    (NormRuleBuilderResult.regular <$> tactic i) <|>
+    normSimpLemmas i <|>
+    (NormRuleBuilderResult.regular <$> apply i) <|>
+    throwError "aesop: Unable to interpret {i} as a normalization rule."
+  | i@(RuleIdent.fvar _) =>
+    throwError "aesop: Please specify a builder for norm rule {i}."
+
+end Aesop.RuleBuilder
