Aesop/Tree.lean
@@ -5,16 +5,17 @@ Authors: Jannis Limperg, Asta Halkjær From
 -/
 
 import Aesop.MutAltTree
-import Aesop.Percent
 import Aesop.Rule
+import Aesop.Util
+import Aesop.Tracing
 
 open Lean
 open Lean.Meta
 
 @[inlineIfReduce]
 private def Bool.toYesNo : Bool → Format
-  | true => "y"
-  | false => "n"
+  | true => "yes"
+  | false => "no "
 
 namespace Aesop
 
@@ -44,8 +45,8 @@ instance : LT GoalId where
 instance : DecidableRel (α := GoalId) (· < ·) :=
   λ n m => inferInstanceAs (Decidable (n.toNat < m.toNat))
 
-instance : ToFormat GoalId where
-  format n := format n.toNat
+instance : ToString GoalId where
+  toString n := toString n.toNat
 
 end GoalId
 
@@ -76,106 +77,138 @@ instance : LT RappId where
 instance : DecidableRel (α := RappId) (· < ·) :=
   λ n m => inferInstanceAs $ Decidable (n.toNat < m.toNat)
 
-instance : ToFormat RappId where
-  format n := format n.toNat
+instance : ToString RappId where
+  toString n := toString n.toNat
 
 end RappId
 
 
 /-! ## Goal Nodes and Rule Applications -/
 
+inductive ProofStatus
+  | unproven
+  | provenByRuleApplication
+  | provenByNormalization
+  deriving Inhabited, BEq
+
+namespace ProofStatus
+
+def isProven : ProofStatus → Bool
+  | unproven => false
+  | provenByRuleApplication => true
+  | provenByNormalization => true
+
+end ProofStatus
+
+
+-- Invariant: if proofStatus = provenByNormalization then isNormal = true
 structure GoalData : Type where
   id : GoalId
   goal : MVarId
   successProbability : Percent
-  normalizationProof : Option Expr
   failedRapps : List RegularRule
   unsafeQueue : Option (List UnsafeRule)
-  proven? : Bool
-  unprovable? : Bool
-  irrelevant? : Bool
+  proofStatus : ProofStatus
+  isUnprovable : Bool
+  isIrrelevant : Bool
+  isNormal : Bool
   deriving Inhabited
 
 namespace GoalData
 
-def normal? (g : GoalData) : Bool :=
-  g.normalizationProof.isSome
+def isProven (g : GoalData) : Bool :=
+  g.proofStatus.isProven
 
-structure MessageInfo where
+protected structure MessageInfo where
   showGoal : Bool
   showUnsafeQueue : Bool
   showFailedRapps : Bool
   deriving Inhabited
 
+open GoalData (MessageInfo)
+
+protected def getMessageInfo [Monad m] [MonadOptions m]
+    (traceCtx : TraceContext) : m MessageInfo := do
+  return {
+    showGoal := (← TraceOption.showGoals.get traceCtx)
+    showUnsafeQueue := (← TraceOption.showUnsafeQueues.get traceCtx)
+    showFailedRapps := (← TraceOption.showFailedRapps.get traceCtx)
+  }
+
 open MessageData in
-protected def toMessageData (minfo : MessageInfo) (g : GoalData) : MessageData :=
+protected def toMessageData (traceCtx : TraceContext) (g : GoalData) :
+    MetaM MessageData := do
+  let minfo ← GoalData.getMessageInfo traceCtx
   let unsafeQueueLength :=
     match g.unsafeQueue with
     | none => f!"<not selected>"
     | some q => format q.length
-  m!"Goal {g.id} [{g.successProbability}]" ++ indentDUnlinesSkipEmpty
-    [ m!"Unsafe rules in queue: {unsafeQueueLength}, failed: {g.failedRapps.length}",
-      join
-        [ m!"normal: {g.normal?.toYesNo} | ",
-          m!"proven: {g.proven?.toYesNo} | ",
-          m!"unprovable: {g.unprovable?.toYesNo} | ",
-          m!"irrelevant: {g.irrelevant?.toYesNo}" ],
-      toMessageDataIf minfo.showGoal $
-        m!"Goal:{indentD g.goal}",
-      toMessageDataIf (minfo.showUnsafeQueue && g.unsafeQueue.isSome) $
-        m!"Unsafe queue:{indentDUnlines $ g.unsafeQueue.get!.map toMessageData}",
-      toMessageDataIf minfo.showFailedRapps $
-        m!"Failed rule applications:{indentDUnlines $ g.failedRapps.map toMessageData}" ]
+  return m!"Goal {g.id} [{g.successProbability.toHumanString}]" ++ nodeFiltering #[
+    m!"Unsafe rules in queue: {unsafeQueueLength}, failed: {g.failedRapps.length}",
+    join
+      [ m!"normal: {g.isNormal.toYesNo} | ",
+        m!"proven: {g.isProven.toYesNo} | ",
+        m!"unprovable: {g.isUnprovable.toYesNo} | ",
+        m!"irrelevant: {g.isIrrelevant.toYesNo}" ],
+    if ¬ minfo.showGoal then none else
+      m!"Goal:{indentD $ ofGoal g.goal}",
+    if ¬ minfo.showUnsafeQueue || g.unsafeQueue.isNone then none else
+      m!"Unsafe queue:{indentDUnlines $ g.unsafeQueue.get!.map toMessageData}",
+    if ¬ minfo.showFailedRapps then none else
+      m!"Failed rule applications:{indentDUnlines $ g.failedRapps.map toMessageData}" ]
 
-def mkInitial (id : GoalId) (goal : MVarId) (successProbability : Percent) :
-    GoalData where
+protected def mkInitial (id : GoalId) (goal : MVarId)
+    (successProbability : Percent) : GoalData where
   id := id
   goal := goal
   successProbability := successProbability
-  normalizationProof := none
   failedRapps := []
   unsafeQueue := none
-  proven? := false
-  unprovable? := false
-  irrelevant? := false
+  proofStatus := ProofStatus.unproven
+  isUnprovable := false
+  isIrrelevant := false
+  isNormal := false
 
 end GoalData
 
 structure RappData : Type where
   id : RappId
+  state : Meta.SavedState
+    -- This is the state *after* the rule was successfully applied, so the goal
+    -- mvar is assigned in this state.
   appliedRule : RegularRule
   successProbability : Percent
-  proof : Expr
-  proven? : Bool
-  unprovable? : Bool
-  irrelevant? : Bool
+  isProven : Bool
+  isUnprovable : Bool
+  isIrrelevant : Bool
   deriving Inhabited
 
 namespace RappData
 
-structure MessageInfo where
-  showProof : Bool
+protected structure MessageInfo where
+
+open RappData (MessageInfo)
 
 open MessageData in
-protected def toMessageData (minfo : MessageInfo) (r : RappData) : MessageData :=
-  m!"Rule application {r.id} [{r.successProbability}]" ++ indentDUnlinesSkipEmpty
-    [ toMessageData r.appliedRule,
+protected def toMessageData [Monad m] [MonadOptions m] (traceCtx : TraceContext)
+    (r : RappData) : m MessageData := do
+  return m!"Rapp {r.id} [{r.successProbability.toHumanString}]" ++
+    nodeFiltering #[
+      toMessageData r.appliedRule,
       join
-        [ m!"proven: {r.proven?.toYesNo} | ",
-          m!"unprovable: {r.unprovable?.toYesNo} | ",
-          m!"irrelevant: {r.irrelevant?.toYesNo}" ],
-      toMessageDataIf minfo.showProof $
-        m!"Proof:{indentD r.proof}" ]
+        [ m!"proven: {r.isProven.toYesNo} | ",
+          m!"unprovable: {r.isUnprovable.toYesNo} | ",
+          m!"irrelevant: {r.isIrrelevant.toYesNo}" ] ]
 
-def mkInitial (id : RappId) (appliedRule : RegularRule)
-  (successProbability : Percent) (proof : Expr) : RappData where
+protected def mkInitial (id : RappId) (state : Meta.SavedState)
+    (appliedRule : RegularRule) (successProbability : Percent) : RappData where
   id := id
+  state := state
   appliedRule := appliedRule
   successProbability := successProbability
-  proof := proof
-  proven? := false
-  unprovable? := false
-  irrelevant? := false
+  isProven := false
+  isUnprovable := false
+  isIrrelevant := false
 
 end RappData
 
@@ -185,7 +218,8 @@ abbrev GoalRef := IO.Ref Goal
 abbrev Rapp    := MutAltTree IO.RealWorld RappData GoalData
 abbrev RappRef := IO.Ref Rapp
 
-variable {m} [Monad m] [MonadLiftT (ST IO.RealWorld) m]
+variable [Monad m] [MonadLiftT (ST IO.RealWorld) m]
+
 
 /-! ## Functions on Goals -/
 
@@ -194,7 +228,7 @@ namespace Goal
 /-! ### Constructors -/
 
 @[inline]
-def mk (parent : Option RappRef) (rapps : Array RappRef)
+protected def mk (parent : Option RappRef) (rapps : Array RappRef)
     (data : GoalData) : Goal :=
   MutAltTree.mk data parent rapps
 
@@ -217,10 +251,6 @@ def successProbability (g : Goal) : Percent :=
   g.payload.successProbability
 
 @[inline]
-def normalizationProof (g : Goal) : Option Expr :=
-  g.payload.normalizationProof
-
-@[inline]
 def failedRapps (g : Goal) : List RegularRule :=
   g.payload.failedRapps
 
@@ -229,16 +259,24 @@ def unsafeQueue (g : Goal) : Option (List UnsafeRule) :=
   g.payload.unsafeQueue
 
 @[inline]
-def proven? (g : Goal) : Bool :=
-  g.payload.proven?
+def proofStatus (g : Goal) : ProofStatus :=
+  g.payload.proofStatus
 
 @[inline]
-def unprovable? (g : Goal) : Bool :=
-  g.payload.unprovable?
+def isProven (g : Goal) : Bool :=
+  g.payload.isProven
 
 @[inline]
-def irrelevant? (g : Goal) : Bool :=
-  g.payload.irrelevant?
+def isUnprovable (g : Goal) : Bool :=
+  g.payload.isUnprovable
+
+@[inline]
+def isIrrelevant (g : Goal) : Bool :=
+  g.payload.isIrrelevant
+
+@[inline]
+def isNormal (g : Goal) : Bool :=
+  g.payload.isNormal
 
 /-! ### Setters -/
 
@@ -255,10 +293,6 @@ def setSuccessProbability (successProbability : Percent) (g : Goal) : Goal :=
   g.modifyPayload λ d => { d with successProbability := successProbability }
 
 @[inline]
-def setNormalizationProof (normalizationProof : Expr) (g : Goal) : Goal :=
-  g.modifyPayload λ d => { d with normalizationProof := normalizationProof }
-
-@[inline]
 def setFailedRapps (failedRapps : List RegularRule) (g : Goal) : Goal :=
   g.modifyPayload λ d => { d with failedRapps := failedRapps }
 
@@ -267,22 +301,22 @@ def setUnsafeQueue (unsafeQueue : Option (List UnsafeRule)) (g : Goal) : Goal :=
   g.modifyPayload λ d => { d with unsafeQueue := unsafeQueue }
 
 @[inline]
-def setProven? (proven? : Bool) (g : Goal) : Goal :=
-  g.modifyPayload λ d => { d with proven? := proven? }
+def setProofStatus (proven? : ProofStatus) (g : Goal) : Goal :=
+  g.modifyPayload λ d => { d with proofStatus := proven? }
 
 @[inline]
-def setUnprovable? (unprovable? : Bool) (g : Goal) : Goal :=
-  g.modifyPayload λ d => { d with unprovable? := unprovable? }
+def setUnprovable (unprovable? : Bool) (g : Goal) : Goal :=
+  g.modifyPayload λ d => { d with isUnprovable := unprovable? }
 
 @[inline]
-def setIrrelevant? (irrelevant? : Bool) (g : Goal) : Goal :=
-  g.modifyPayload λ d => { d with irrelevant? := irrelevant? }
+def setIrrelevant (irrelevant? : Bool) (g : Goal) : Goal :=
+  g.modifyPayload λ d => { d with isIrrelevant := irrelevant? }
+
+@[inline]
+def setNormal (normal? : Bool) (g : Goal) : Goal :=
+  g.modifyPayload λ d => { d with isNormal := normal? }
 
 /-! ### Miscellaneous -/
-
-@[inline]
-def normal? (g : Goal) : Bool :=
-  g.payload.normal?
 
 def hasNoUnexpandedUnsafeRule (g : Goal) : Bool :=
   match g.unsafeQueue with
@@ -299,11 +333,17 @@ namespace Rapp
 /-! ### Constructors -/
 
 @[inline]
-def mk (parent : Option GoalRef) (subgoals : Array GoalRef)
+protected def mk (parent : Option GoalRef) (subgoals : Array GoalRef)
     (data : RappData) : Rapp :=
   MutAltTree.mk data parent subgoals
 
 /-! ### Getters -/
+
+@[inline]
+def parent! (r : Rapp) : GoalRef :=
+  match r.parent with
+  | some p => p
+  | none => panic! s!"aesop/Rapp.parent!: rapp {r.payload.id} "
 
 @[inline]
 def subgoals (r : Rapp) : Array GoalRef :=
@@ -314,6 +354,10 @@ def id (r : Rapp) : RappId :=
   r.payload.id
 
 @[inline]
+def state (r : Rapp) : Meta.SavedState :=
+  r.payload.state
+
+@[inline]
 def appliedRule (r : Rapp) : RegularRule :=
   r.payload.appliedRule
 
@@ -322,26 +366,26 @@ def successProbability (r : Rapp) : Percent :=
   r.payload.successProbability
 
 @[inline]
-def proof (r : Rapp) : Expr :=
-  r.payload.proof
+def isProven (r : Rapp) : Bool :=
+  r.payload.isProven
 
 @[inline]
-def proven? (r : Rapp) : Bool :=
-  r.payload.proven?
+def isUnprovable (r : Rapp) : Bool :=
+  r.payload.isUnprovable
 
 @[inline]
-def unprovable? (r : Rapp) : Bool :=
-  r.payload.unprovable?
-
-@[inline]
-def irrelevant? (r : Rapp) : Bool :=
-  r.payload.irrelevant?
+def isIrrelevant (r : Rapp) : Bool :=
+  r.payload.isIrrelevant
 
 -- Setters
 
 @[inline]
 def setId (id : RappId) (r : Rapp) : Rapp :=
   r.modifyPayload λ r => { r with id := id }
+
+@[inline]
+def setState (state : Meta.SavedState) (r : Rapp) : Rapp :=
+  r.modifyPayload λ r => { r with state := state }
 
 @[inline]
 def setAppliedRule (appliedRule : RegularRule) (r : Rapp) : Rapp :=
@@ -352,55 +396,64 @@ def setSuccessProbability (successProbability : Percent) (r : Rapp) : Rapp :=
   r.modifyPayload λ r => { r with successProbability := successProbability }
 
 @[inline]
-def setProof (proof : Expr) (r : Rapp) : Rapp :=
-  r.modifyPayload λ r => { r with proof := proof }
+def setProven (proven? : Bool) (r : Rapp) : Rapp :=
+  r.modifyPayload λ r => { r with isProven := proven? }
 
 @[inline]
-def setProven? (proven? : Bool) (r : Rapp) : Rapp :=
-  r.modifyPayload λ r => { r with proven? := proven? }
+def setUnprovable (unprovable? : Bool) (r : Rapp) : Rapp :=
+  r.modifyPayload λ r => { r with isUnprovable := unprovable? }
 
 @[inline]
-def setUnprovable? (unprovable? : Bool) (r : Rapp) : Rapp :=
-  r.modifyPayload λ r => { r with unprovable? := unprovable? }
-
-@[inline]
-def setIrrelevant? (irrelevant? : Bool) (r : Rapp) : Rapp :=
-  r.modifyPayload λ r => { r with irrelevant? := irrelevant? }
+def setIrrelevant (irrelevant? : Bool) (r : Rapp) : Rapp :=
+  r.modifyPayload λ r => { r with isIrrelevant := irrelevant? }
 
 /-! ### Miscellaneous -/
 
-def subgoalsProven? (r : Rapp) : m Bool :=
-  r.subgoals.allM λ subgoal => return (← subgoal.get).proven?
+def allSubgoalsProven (r : Rapp) : m Bool :=
+  r.subgoals.allM λ subgoal => return (← subgoal.get).isProven
 
 end Rapp
+
 
 /-! ## Formatting -/
 
 mutual
-  private partial def formatTreeGoal (goalMInfo : GoalData.MessageInfo)
-      (rappMInfo : RappData.MessageInfo) (goal : Goal) : m MessageData := do
-    let goalMsg := goal.payload.toMessageData goalMInfo
+  private partial def formatTreeGoal (traceCtx : TraceContext) (goal : Goal) :
+      MetaM MessageData := do
+    let goalMsg ← goal.payload.toMessageData traceCtx
     let childrenMsgs ← goal.rapps.mapM λ c => do
-      formatTreeRapp goalMInfo rappMInfo (← c.get)
+      formatTreeRapp traceCtx (← c.get)
     return goalMsg ++ indentD (MessageData.node childrenMsgs)
 
-  private partial def formatTreeRapp (goalMInfo : GoalData.MessageInfo)
-      (rappMInfo : RappData.MessageInfo) (rapp : Rapp) : m MessageData := do
-    let rappMsg := rapp.payload.toMessageData rappMInfo
+  private partial def formatTreeRapp (traceCtx : TraceContext) (rapp : Rapp) :
+      MetaM MessageData := do
+    let rappMsg ← rapp.payload.toMessageData TraceContext.tree
     let childrenMsgs ← rapp.subgoals.mapM λ c => do
-      formatTreeGoal goalMInfo rappMInfo (← c.get)
+      formatTreeGoal traceCtx (← c.get)
     return rappMsg ++ indentD (MessageData.node childrenMsgs)
 end
 
-@[inline]
-def Goal.formatTree : GoalData.MessageInfo → RappData.MessageInfo → Goal →
-    m MessageData :=
-  formatTreeGoal
+namespace Goal
 
-@[inline]
-def Rapp.formatTree : GoalData.MessageInfo → RappData.MessageInfo → Rapp →
-    m MessageData :=
-  formatTreeRapp
+def toMessageData (traceCtx : TraceContext) (g : Goal) : MetaM MessageData :=
+  g.payload.toMessageData traceCtx
+
+def treeToMessageData (traceCtx : TraceContext) (g : Goal) : MetaM MessageData :=
+  formatTreeGoal traceCtx g
+
+end Goal
+
+namespace Rapp
+
+def toMessageData (traceCtx : TraceContext) (r : Rapp) : MetaM MessageData :=
+  r.payload.toMessageData traceCtx
+
+def treeToMessageData (traceCtx : TraceContext) (r : Rapp) :
+    MetaM MessageData := do
+  formatTreeRapp traceCtx r
+
+end Rapp
+
 
 /-! ## Miscellaneous Functions on Goals -/
 
@@ -411,94 +464,70 @@ def mayHaveUnexpandedRapp (g : Goal) : m Bool := do pure $
   ¬ (← g.rapps.anyM λ r => return (← r.get : Rapp).appliedRule.isSafe)
 
 def hasProvableRapp (g : Goal) : m Bool :=
-  g.rapps.anyM λ r => return ¬ (← r.get).unprovable?
+  g.rapps.anyM λ r => return ¬ (← r.get).isUnprovable
+
+def firstProvenRapp? (g : Goal) : m (Option RappRef) :=
+  g.rapps.findSomeM? λ rref =>
+    return if (← rref.get).isProven then some rref else none
 
 end Goal
 
 
-/-! ## Proof Extraction -/
-
-namespace GoalRef
-
-/- May only be called *once*. The given goal must be proven. -/
-partial def linkProofs (gref : GoalRef) : MetaM Unit := do
-  let g ← gref.get
-  let (some r) ← g.rapps.findSomeM? λ r => do
-    let r ← r.get
-    return if r.proven? then some r else none
-    | throwError "aesop/linkProofs: internal error: node {g.id} not proven"
-  r.subgoals.forM linkProofs
-  let goalMVar := g.goal
-  checkNotAssigned `aesop goalMVar
-  -- TODO check for type-correct assignment?
-  -- let goalType ← getMVarType goalMVar
-  -- let (true) ← isDefEq goalType r.proof | throwError
-  --   "aesop/linkProofs: internal error: proof of rule application {r.id} did not unify with the goal of its parent node {g.id}"
-  assignExprMVar g.goal r.proof
-
-/- Only call this after `linkProofs` has been run. -/
-def extractProof (gref : GoalRef) : MetaM Expr := do
-  let g ← gref.get
-  match g.normalizationProof with
-  | none => instantiateMVars $ mkMVar g.goal
-  | some prf => instantiateMVars prf
-
-end GoalRef
-
 /-! ## Propagating Provability/Unprovability/Irrelevance -/
 
 @[inline]
-def Internal.setIrrelevant : Sum GoalRef RappRef → m Unit :=
+def setIrrelevantImpl : Sum GoalRef RappRef → m Unit :=
   MutAltTree.visitDown'
     (λ gref => do
       let g : Goal ← gref.get
-      if g.irrelevant?
+      if g.isIrrelevant
         then return false -- Subtree should already be marked as irrelevant.
         else do
-          gref.set $ g.setIrrelevant? true
+          gref.set $ g.setIrrelevant true
           return true)
     (λ rref => do
       let r : Rapp ← rref.get
-      if r.irrelevant?
+      if r.isIrrelevant
         then return false
         else do
-          rref.set $ r.setIrrelevant? true
+          rref.set $ r.setIrrelevant true
           return true)
 
 def GoalRef.setIrrelevant : GoalRef → m Unit :=
-  Internal.setIrrelevant ∘ Sum.inl
+  setIrrelevantImpl ∘ Sum.inl
 
 def RappRef.setIrrelevant : RappRef → m Unit :=
-  Internal.setIrrelevant ∘ Sum.inr
+  setIrrelevantImpl ∘ Sum.inr
 
 @[inline]
-def Internal.setProven : Sum GoalRef RappRef → m Unit :=
+private def setProvenImpl : Sum GoalRef RappRef → m Unit :=
   MutAltTree.visitUp'
     -- Goals are unconditionally marked as proven.
     (λ gref => do
-      gref.modify λ (g : Goal) => g.setProven? true
+      gref.modify λ (g : Goal) =>
+        g.setProofStatus ProofStatus.provenByRuleApplication
       return true)
     -- Rapps are marked as proven only if they are in fact proven, i.e. if all
     -- their subgoals are (marked as) proven. In this case, we also need to
     -- mark siblings of the rapp (and their descendants) as irrelevant.
     (λ rref => do
       let r : Rapp ← rref.get
-      if ¬ (← r.subgoalsProven?)
+      if ¬ (← r.allSubgoalsProven)
         then return false
         else do
-          rref.set $ r.setProven? true
+          rref.set $ r.setProven true
           let siblings ← MutAltTree.siblings rref
           siblings.forM RappRef.setIrrelevant
           return true)
 
 def GoalRef.setProven : GoalRef → m Unit :=
-  Internal.setProven ∘ Sum.inl
+  setProvenImpl ∘ Sum.inl
 
 def RappRef.setProven : RappRef → m Unit :=
-  Internal.setProven ∘ Sum.inr
+  setProvenImpl ∘ Sum.inr
 
 @[inline]
-def Internal.setUnprovable : Sum GoalRef RappRef → m Unit :=
+private def setUnprovableImpl : Sum GoalRef RappRef → m Unit :=
   MutAltTree.visitUp'
     -- Goals are marked as unprovable only if they are in fact unprovable, i.e.
     -- if all their rule applications are unprovable and they do not have
@@ -509,19 +538,19 @@ def Internal.setUnprovable : Sum GoalRef RappRef → m Unit :=
       if (← g.mayHaveUnexpandedRapp <||> g.hasProvableRapp)
         then return false
         else do
-          gref.set $ g.setUnprovable? true
+          gref.set $ g.setUnprovable true
           let siblings ← MutAltTree.siblings gref
           siblings.forM GoalRef.setIrrelevant
           return true)
     -- Rapps are unconditionally marked as unprovable.
     (λ rref => do
-      rref.modify λ (r : Rapp) => r.setUnprovable? true
+      rref.modify λ (r : Rapp) => r.setUnprovable true
       return true)
 
 def GoalRef.setUnprovable : GoalRef → m Unit :=
-  Internal.setUnprovable ∘ Sum.inl
+  setUnprovableImpl ∘ Sum.inl
 
 def RappRef.setUnprovable : RappRef → m Unit :=
-  Internal.setUnprovable ∘ Sum.inr
+  setUnprovableImpl ∘ Sum.inr
 
 end Aesop
