Aesop/Config.lean
@@ -1,0 +1,479 @@
+/-
+Copyright (c) 2021 Jannis Limperg. All rights reserved.
+Released under Apache 2.0 license as described in the file LICENSE.
+Authors: Jannis Limperg, Asta Halkjær From
+-/
+
+import Aesop.RuleBuilder
+
+open Lean
+open Lean.Meta (SimpEntry getSimpLemmas)
+
+namespace Aesop
+
+namespace Parser.Attribute
+
+declare_syntax_cat aesop_prio
+
+syntax "-"? num "%"? : aesop_prio
+
+declare_syntax_cat' aesop_kind force_leading_unreserved_tokens
+
+syntax (aesop_prio)? : aesop_kind
+syntax &"safe" (aesop_prio)? : aesop_kind
+syntax &"unsafe" (aesop_prio)? : aesop_kind
+syntax &"norm" (aesop_prio)? : aesop_kind
+
+declare_syntax_cat' aesop_builder force_leading_unreserved_tokens
+
+syntax &"apply" : aesop_builder
+syntax &"simp" : aesop_builder
+syntax &"unfold" : aesop_builder
+syntax &"tactic" : aesop_builder
+
+declare_syntax_cat' aesop_clause force_leading_unreserved_tokens
+
+syntax "(" &"builder" aesop_builder ")" : aesop_clause
+
+syntax (name := aesop) &"aesop" aesop_kind aesop_clause* : attr
+
+end Parser.Attribute
+
+
+variable [Monad m] [MonadError m]
+
+
+inductive Prio
+  | successProbability (p : Percent)
+  | penalty (i : Int)
+  deriving Inhabited, BEq
+
+namespace Prio
+
+instance : ToString Prio where
+  toString
+    | successProbability p => p.toHumanString
+    | penalty i => toString i
+
+protected def parse : Syntax → Except String Prio
+  | `(aesop_prio|- $n:numLit %) =>
+    throw "percentage cannot be negative"
+  | `(aesop_prio|- $n:numLit) => return penalty $ - n.toNat
+  | `(aesop_prio|$n:numLit) => return penalty $ n.toNat
+  | `(aesop_prio|$n:numLit %) => do
+    let (some p) ← Percent.ofNat n.toNat
+      | throw "percentage must be between 0 and 100."
+    return successProbability p
+  | _ => unreachable!
+
+end Prio
+
+def parsePrioForUnsafeRule : Option Syntax → Except String Percent
+  | none => throw "unsafe rule must be given a success probability."
+  | some p => do
+    let (Prio.successProbability p) ← Prio.parse p | throw
+      "unsafe rule must be given a success probability ('x%'), not an integer penalty"
+    return p
+
+def parsePrioForSafeRule : Option Syntax → Except String Int
+  | none => return defaultSafePenalty
+  | some p => do
+    let (Prio.penalty p) ← Prio.parse p | throw
+      "safe rule must be given an integer penalty, not a success probability"
+    return p
+
+def parsePrioForNormRule : Option Syntax → Except String Int
+  | none => return defaultNormPenalty
+  | some p => do
+    let (Prio.penalty p) ← Prio.parse p | throw
+      "norm rule must be given an integer penalty, not a success probability"
+    return p
+
+inductive RuleKind
+  | norm (penalty : Int)
+  | safe (penalty : Int)
+  | «unsafe» (successProbability : Percent)
+  deriving Inhabited, BEq
+
+namespace RuleKind
+
+instance : ToString RuleKind where
+  toString
+    | norm p => s!"norm {p}"
+    | safe p => s!"safe {p}"
+    | «unsafe» p => s!"unsafe {p.toHumanString}"
+
+protected def parse : Syntax → m RuleKind
+  | `(aesop_kind|safe $[$prio:aesop_prio]?) =>
+    go (parsePrioForSafeRule prio) safe
+  | `(aesop_kind|unsafe $[$prio:aesop_prio]?) =>
+    go (parsePrioForUnsafeRule prio) «unsafe»
+  | `(aesop_kind|$[$prio:aesop_prio]?) =>
+    go (parsePrioForUnsafeRule prio) «unsafe»
+  | `(aesop_kind|norm $[$prio:aesop_prio]?) =>
+    go (parsePrioForNormRule prio) norm
+  | _ => unreachable!
+  where
+    go {α} (prio : Except String α) (cont : α → RuleKind) : m RuleKind :=
+      match prio with
+      | Except.ok prio => return cont prio
+      | Except.error e => throwError "aesop: {e}"
+
+end RuleKind
+
+
+inductive RegularBuilderClause
+  | apply
+  | tactic
+  deriving Inhabited, BEq
+
+namespace RegularBuilderClause
+
+instance : ToString RegularBuilderClause where
+  toString
+    | apply => "(builder apply)"
+    | tactic => "(builder tactic)"
+
+def toRuleBuilder : RegularBuilderClause → RuleBuilder RegularRuleBuilderResult
+  | apply => RuleBuilder.apply
+  | tactic => RuleBuilder.tactic
+
+end RegularBuilderClause
+
+
+inductive BuilderClause
+  | regular (c : RegularBuilderClause)
+  | simpLemma
+  | simpUnfold
+  deriving Inhabited, BEq
+
+namespace BuilderClause
+
+instance : ToString BuilderClause where
+  toString
+    | regular c => toString c
+    | simpLemma => "(builder simp)"
+    | simpUnfold => "(builder unfold)"
+
+open RegularBuilderClause in
+protected def parseBuilder : Syntax → BuilderClause
+  | `(aesop_builder|apply) => regular apply
+  | `(aesop_builder|tactic) => regular tactic
+  | `(aesop_builder|simp) => simpLemma
+  | `(aesop_builder|unfold) => simpUnfold
+  | _ => unreachable!
+
+def toRuleBuilder : BuilderClause → RuleBuilder NormRuleBuilderResult
+  | regular c => λ goal i =>
+    NormRuleBuilderResult.regular <$> c.toRuleBuilder goal i
+  | simpLemma => RuleBuilder.normSimpLemmas
+  | simpUnfold => RuleBuilder.normSimpUnfold
+
+end BuilderClause
+
+
+inductive Clause
+  | builder (c : BuilderClause)
+  deriving Inhabited, BEq
+
+namespace Clause
+
+instance : ToString Clause where
+  toString
+    | builder c => toString c
+
+protected def parse : Syntax → m Clause
+  | `(aesop_clause|(builder $b:aesop_builder)) =>
+    builder <$> BuilderClause.parseBuilder b
+  | _ => unreachable!
+
+end Clause
+
+
+structure NormRuleConfig where
+  penalty : Option Int
+  builder : Option BuilderClause
+  deriving Inhabited, BEq
+
+namespace NormRuleConfig
+
+instance : ToString NormRuleConfig where
+  toString conf :=
+    " ".joinSep
+      [ match conf.penalty with | none => "" | some p => toString p,
+        match conf.builder with | none => "" | some b => toString b ]
+
+protected def addClause (conf : NormRuleConfig) :
+    Clause → m NormRuleConfig
+  | Clause.builder b =>
+    if conf.builder.isSome
+      then throwError "aesop: duplicate builder clause."
+      else pure { conf with builder := b }
+
+protected def addClauses (clauses : Array Clause)
+    (conf : NormRuleConfig) : m NormRuleConfig :=
+  clauses.foldlM NormRuleConfig.addClause conf
+
+open NormRuleBuilderResult in
+protected def applyToRuleIdent (i : RuleIdent)
+    (conf : NormRuleConfig) : MetaM RuleSetMember := do
+  let builderResult ←
+    match conf.builder with
+    | none => RuleBuilder.normRuleDefault i
+    | some builderClause => builderClause.toRuleBuilder i
+  match builderResult with
+  | regular res =>
+    let penalty := conf.penalty.getD 1
+    return RuleSetMember'.normRule
+      { name := `norm ++ res.builderName ++ i.ruleName
+        indexingMode := res.indexingMode
+        extra := { penalty := penalty }
+        tac := res.tac }
+  | simpEntries es =>
+    return RuleSetMember'.normSimpEntries es
+
+end NormRuleConfig
+
+
+structure SafeRuleConfig where
+  penalty : Option Int
+  builder : Option RegularBuilderClause
+  deriving Inhabited
+
+namespace SafeRuleConfig
+
+instance : ToString SafeRuleConfig where
+  toString conf :=
+    " ".joinSep
+      [ match conf.penalty with | none => "" | some p => toString p,
+        match conf.builder with
+          | none => ""
+          | some b => toString (BuilderClause.regular b) ]
+
+protected def addClause (conf : SafeRuleConfig) : Clause → m SafeRuleConfig
+  | Clause.builder BuilderClause.simpLemma =>
+    throwError "aesop: 'simp' builder cannot be used with safe rules."
+  | Clause.builder BuilderClause.simpUnfold =>
+    throwError "aesop: 'unfold' builder cannot be used with safe rules."
+  | Clause.builder (BuilderClause.regular b) =>
+    if conf.builder.isSome
+      then throwError "aesop: duplicate builder clause."
+      else pure { conf with builder := b }
+
+protected def addClauses (clauses : Array Clause) (conf : SafeRuleConfig) :
+    m SafeRuleConfig :=
+  clauses.foldlM SafeRuleConfig.addClause conf
+
+protected def applyToRuleIdent (i : RuleIdent)
+    (conf : SafeRuleConfig) : MetaM RuleSetMember := do
+  let builderResult ←
+    match conf.builder with
+    | none => RuleBuilder.safeRuleDefault i
+    | some builderClause => builderClause.toRuleBuilder i
+  let penalty := conf.penalty.getD 0
+  return RuleSetMember'.safeRule
+    { name := `safe ++ builderResult.builderName ++ i.ruleName
+      indexingMode := builderResult.indexingMode,
+      extra := { penalty := penalty, safety := Safety.safe }
+        -- TODO support almost_safe rules
+      tac := builderResult.tac }
+
+end SafeRuleConfig
+
+
+structure UnsafeRuleConfig where
+  successProbability : Percent
+  builder : Option RegularBuilderClause
+  deriving Inhabited
+
+namespace UnsafeRuleConfig
+
+instance : ToString UnsafeRuleConfig where
+  toString conf :=
+    " ".joinSep
+      [ conf.successProbability.toHumanString,
+        match conf.builder with
+          | none => ""
+          | some b => toString (BuilderClause.regular b) ]
+
+protected def addClause (conf : UnsafeRuleConfig) : Clause → m UnsafeRuleConfig
+  | Clause.builder BuilderClause.simpLemma =>
+    throwError "aesop: 'simp' builder cannot be used with unsafe rules."
+  | Clause.builder BuilderClause.simpUnfold =>
+    throwError "aesop: 'unfold' builder cannot be used with unsafe rules."
+  | Clause.builder (BuilderClause.regular b) =>
+    if conf.builder.isSome
+      then throwError "aesop: duplicate builder clause."
+      else pure { conf with builder := b }
+
+protected def addClauses (clauses : Array Clause) (conf : UnsafeRuleConfig) :
+    m UnsafeRuleConfig :=
+  clauses.foldlM UnsafeRuleConfig.addClause conf
+
+protected def applyToRuleIdent (i : RuleIdent) (conf : UnsafeRuleConfig) :
+    MetaM RuleSetMember := do
+  let builderResult ←
+    match conf.builder with
+    | none => RuleBuilder.unsafeRuleDefault i
+    | some builderClause => builderClause.toRuleBuilder i
+  return RuleSetMember'.unsafeRule
+    { name := `unsafe ++ builderResult.builderName ++ i.ruleName
+      indexingMode := builderResult.indexingMode,
+      extra := { successProbability := conf.successProbability },
+      tac := builderResult.tac }
+
+end UnsafeRuleConfig
+
+
+inductive RuleConfig
+  | norm (conf : NormRuleConfig)
+  | safe (conf : SafeRuleConfig)
+  | «unsafe» (conf : UnsafeRuleConfig)
+  deriving Inhabited
+
+namespace RuleConfig
+
+instance : ToString RuleConfig where
+  toString c :=
+    "aesop " ++
+    match c with
+      | norm conf => " ".joinSep ["norm", toString conf]
+      | safe conf => " ".joinSep ["safe", toString conf]
+      | «unsafe» conf => " ".joinSep ["unsafe", toString conf]
+
+protected def ofKindAndClauses : RuleKind → Array Clause → m RuleConfig
+  | RuleKind.norm penalty, cs => do
+    let conf : NormRuleConfig := { penalty := penalty, builder := none }
+    norm <$> conf.addClauses cs
+  | RuleKind.safe penalty, cs => do
+    let conf : SafeRuleConfig := { penalty := penalty, builder := none }
+    safe <$> conf.addClauses cs
+  | RuleKind.unsafe prob, cs => do
+    let conf : UnsafeRuleConfig := { successProbability := prob, builder := none }
+    «unsafe» <$> conf.addClauses cs
+
+protected def parse : Syntax → m RuleConfig
+  | `(attr|aesop $kind:aesop_kind $[$clauses:aesop_clause]*) => do
+    let kind ← RuleKind.parse kind
+    let clauses ← clauses.mapM Clause.parse
+    RuleConfig.ofKindAndClauses kind clauses
+  | _ => unreachable!
+
+protected def applyToRuleIdent (i : RuleIdent) :
+  RuleConfig → MetaM RuleSetMember
+  | norm conf => conf.applyToRuleIdent i
+  | safe conf => conf.applyToRuleIdent i
+  | «unsafe» conf => conf.applyToRuleIdent i
+
+end RuleConfig
+
+structure AesopAttr where
+  ext : ScopedEnvExtension (RuleSetMember' RuleTacDescr) RuleSetMember RuleSet
+  impl : AttributeImpl
+  deriving Inhabited
+
+initialize attr : AesopAttr ← do
+  let ext ← registerScopedEnvExtension {
+    name := `aesop
+    mkInitial := return {}
+    ofOLeanEntry := λ rs r => runMetaMAsImportM r.ofDescr
+    toOLeanEntry := λ r => r.toDescr.getD
+      (panic! "aesop attribute extension: trying to serialise a rule set member without a description")
+    addEntry := λ rs r => rs.add r
+  }
+  let impl : AttributeImpl := {
+    name := `aesop
+    descr := "Register a declaration as an Aesop rule."
+    add := λ decl stx attrKind => do
+      let config ← RuleConfig.parse stx
+      let rule ← runMetaMAsCoreM $ config.applyToRuleIdent (RuleIdent.const decl)
+      ext.add rule attrKind
+    erase := λ _ =>
+      throwError "aesop attribute currently cannot be removed"
+  }
+  -- Despite the name, this also works for non-builtin attributes.
+  registerBuiltinAttribute impl
+  pure { ext := ext, impl := impl }
+
+def getAttrRuleSet : CoreM RuleSet := do
+  attr.ext.getState (← getEnv)
+
+def getRuleSet : MetaM RuleSet := do
+  let defaultSimpLemmas ← getSimpLemmas
+  let rs ← getAttrRuleSet
+  return { rs with normSimpLemmas := defaultSimpLemmas.merge rs.normSimpLemmas }
+
+
+namespace Parser.Tactic
+
+declare_syntax_cat aesop_rule
+
+syntax ident (aesop_prio)? (aesop_clause)* : aesop_rule
+
+declare_syntax_cat aesop_tactic_clause
+
+syntax ruleList := "[" aesop_rule,+,? "]"
+
+syntax "(" &"unsafe" ruleList ")" : aesop_tactic_clause
+syntax "(" &"safe"   ruleList ")" : aesop_tactic_clause
+syntax "(" &"norm"   ruleList ")" : aesop_tactic_clause
+
+syntax (name := aesop) &"aesop " (aesop_tactic_clause)* : tactic
+
+end Parser.Tactic
+
+structure AdditionalRule where
+  ruleIdent : RuleIdent
+  config : RuleConfig
+  deriving Inhabited
+
+namespace AdditionalRule
+
+protected def parse (prioParser : Option Syntax → Except String α)
+    (ruleKind : α → RuleKind) : Syntax → MetaM AdditionalRule
+  | `(aesop_rule|$i:ident $[$prio:aesop_prio]? $clauses:aesop_clause*) => do
+    let prio ←
+      match prioParser prio with
+      | Except.ok p => p
+      | Except.error e => throwError "aesop: at rule {i}: {e}"
+    let clauses ← clauses.mapM Clause.parse
+    let config ← RuleConfig.ofKindAndClauses (ruleKind prio) clauses
+    return { ruleIdent := (← RuleIdent.ofName i.getId), config := config }
+  | _ => unreachable!
+
+protected def toRuleSetMember (r : AdditionalRule) : MetaM RuleSetMember :=
+  r.config.applyToRuleIdent r.ruleIdent
+
+end AdditionalRule
+
+def parseAdditionalRuleClause : Syntax → MetaM (Array AdditionalRule)
+  | `(aesop_tactic_clause|(unsafe [$rules:aesop_rule,*])) =>
+    (rules : Array Syntax).mapM
+      (AdditionalRule.parse parsePrioForUnsafeRule RuleKind.unsafe)
+  | `(aesop_tactic_clause|(safe [$rules:aesop_rule,*])) =>
+    (rules : Array Syntax).mapM
+      (AdditionalRule.parse parsePrioForSafeRule RuleKind.safe)
+  | `(aesop_tactic_clause|(norm [$rules:aesop_rule,*])) =>
+    (rules : Array Syntax).mapM
+      (AdditionalRule.parse parsePrioForNormRule RuleKind.norm)
+  | _ => unreachable!
+
+structure TacticConfig where
+  additionalRules : Array AdditionalRule
+  deriving Inhabited
+
+namespace TacticConfig
+
+-- NOTE: Must be called with the MVar context of the main goal.
+protected def parse : Syntax → MetaM TacticConfig
+  | `(tactic|aesop $[$clauses:aesop_tactic_clause]*) => do
+    let rs ← clauses.concatMapM parseAdditionalRuleClause
+    return { additionalRules := rs }
+  | _ => unreachable!
+
+def additionalRuleSetMembers (c : TacticConfig) : MetaM (Array RuleSetMember) :=
+  c.additionalRules.mapM (·.toRuleSetMember)
+
+end TacticConfig
+
+end Aesop
