Aesop/DefaultRules.lean
@@ -1,0 +1,45 @@
+/-
+Copyright (c) 2021 Jannis Limperg. All rights reserved.
+Released under Apache 2.0 license as described in the file LICENSE.
+Authors: Jannis Limperg
+-/
+
+import Aesop.DefaultRules.SplitHyps
+import Aesop.Config
+
+open Lean
+open Lean.Elab
+open Lean.Elab.Tactic
+
+namespace Aesop.DefaultRules
+
+def assumption : TacticM Unit :=
+  liftMetaTactic λ goal => Lean.Meta.assumption goal *> pure []
+
+def intros : TacticM Unit := do
+  evalTactic (← `(tactic|intros))
+
+def splitHyps : TacticM Unit :=
+  liftMetaTactic λ goal => return [(← splitAllHyps goal).snd]
+
+end DefaultRules
+
+-- We could tag the above rule defs with the aesop attribute, and that would
+-- certainly be more convenient than what this function does. However, the
+-- attribute would come from the stage0 library, so any change to e.g.
+-- the attribute syntax would require a stage0 update. These updates are a major
+-- PITA when we rebase onto upstream master, so we want to minimise them.
+def defaultRules : TermElabM (Array RuleSetMember) := do
+  mkRules #[
+    (``DefaultRules.assumption, ← `(attr|aesop safe 0)),
+    (``DefaultRules.intros    , ← `(attr|aesop norm -1)),
+    (``DefaultRules.splitHyps , ← `(attr|aesop norm 0)) ]
+  where
+    mkRule (decl : Name) (configStx : Syntax) : TermElabM RuleSetMember := do
+      let config ← RuleConfig.parse configStx
+      config.applyToRuleIdent (RuleIdent.const decl)
+
+    mkRules (rs : Array (Name × Syntax)) : TermElabM (Array RuleSetMember) :=
+      rs.mapM (λ (decl, configStx) => mkRule decl configStx)
+
+end Aesop
