Aesop/DefaultRules/SplitHyps.lean
@@ -1,0 +1,185 @@
+/-
+Copyright (c) 2021 Jannis Limperg. All rights reserved.
+Released under Apache 2.0 license as described in the file LICENSE.
+Authors: Jannis Limperg
+-/
+import Lean.Elab.Tactic
+
+open Lean
+
+namespace Aesop.DefaultRules
+
+-- We define the `splitHyp` tactic, which splits hypotheses that are products
+-- or existentials. It recurses into nested products, so `A ∧ B ∧ C` is split
+-- into three hypotheses with types `A`, `B` and `C`. It also works under
+-- binders, so `h : ∀ x, P x ∧ Q x` is split into `h₁ : ∀ x, P x` and
+-- `h₂ : ∀ x, Q x`.
+--
+-- Exception: `Exists`, unlike `Sigma` and `PSigma`, cannot be split under
+-- binders. This is unavoidable: `∀ (x : X), ∃ (y : Y), P y` does not imply
+-- `∃ (f : X → Y), ∀ x, P (f x)` in Lean's logic.
+
+-- TODO The splitHyps tactic currently does not handle existentials with
+-- products nested in the witness. E.g. the hypothesis
+--
+--   h : ∃ (p : X × Y), P p
+--
+-- is decomposed into
+--
+--   h₁ : X × Y
+--   h₂ : P h₁
+--
+-- when it should really be
+--
+--   h₁ : X
+--   h₂ : Y
+--   h₃ : P (h₁, h₂)
+--
+-- To fix this, we should canonicalise such hypotheses before splitting them.
+-- The canonicalisation would make sure the witness is not a product by
+-- rewriting, e.g.,
+--
+--   ∃ (p : X × Y), P p           ↝ ∃ (x : X) (y : Y), P (x, y)
+--   ∃ (p : ∃ (x : X), P x), Q p  ↝ ∃ (x : X) (y : P x), Q (Exists.intro x y)
+--
+-- @[simp]
+-- theorem exists_prod {X Y} (P : X × Y → Prop) :
+--     (∃ (p : X × Y), P p) ↔ ∃ (x : X) (y : Y), P (x, y) :=
+--   Iff.intro
+--     (λ ⟨⟨x, y⟩, Pp⟩ => ⟨x, y, Pp⟩)
+--     (λ ⟨x, y, Pxy⟩ => ⟨⟨x, y⟩, Pxy⟩)
+--
+-- We could also use this implementation strategy for splitting under binders:
+-- rewrite `∀ x, P x ∧ Q x` into `(∀ x, P x) ∧ (∀ x, Q x)`. This would reduce
+-- the implementation complexity a lot, though at some performance cost.
+
+open Expr
+open Lean.Meta
+
+partial def splitHypCore (goal : MVarId) (originalUserName : Name)
+    (binderFVars : Array Expr) (hyp : FVarId) (type : Expr) :
+    MetaM (Array FVarId × MVarId) :=
+  match type with
+  | forallE .. => do
+    forallTelescope type λ binders conclusion =>
+      splitHypCore goal originalUserName (binderFVars ++ binders) hyp conclusion
+  | app (app (const ``And lvls _) leftType _) rightType _ =>
+    splitProduct goal (mkConst ``And.left lvls) (mkConst ``And.right lvls)
+      leftType rightType
+  | app (app (const ``Prod lvls _) leftType _) rightType _ =>
+    splitProduct goal (mkConst ``Prod.fst lvls) (mkConst ``Prod.snd lvls)
+      leftType rightType
+  | app (app (const ``PProd lvls _) leftType _) rightType _ =>
+    splitProduct goal (mkConst ``PProd.fst lvls) (mkConst ``PProd.snd lvls)
+      leftType rightType
+  | app (app (const ``MProd lvls _) leftType _) rightType _ =>
+    splitProduct goal (mkConst ``MProd.fst lvls) (mkConst ``MProd.snd lvls)
+      leftType rightType
+  | app (app (const ``Sigma lvls _) witnessType _) propertyType _ => do
+    splitExistential goal (mkConst ``Sigma.fst lvls) (mkConst ``Sigma.snd lvls)
+      witnessType propertyType
+  | app (app (const ``PSigma lvls _) witnessType _) propertyType _ => do
+    splitExistential goal (mkConst ``PSigma.fst lvls) (mkConst ``PSigma.snd lvls)
+      witnessType propertyType
+  | app (app (const ``Exists lvls _) witnessType _) propertyType _ => do
+    -- We can't eliminate Exists under binders.
+    if ¬ binderFVars.isEmpty then
+      return (#[], goal)
+    let #[casesGoal] ← cases goal hyp
+      | unreachable!
+    pure (casesGoal.fields.map (·.fvarId!), casesGoal.mvarId)
+  | _ => pure (#[], goal)
+  where
+    hypWithBinderFVars : Expr :=
+      mkAppN (mkFVar hyp) binderFVars
+
+    splitProductHalf (goal : MVarId) (left : Bool)
+        (eliminator leftType rightType : Expr) : MetaM (FVarId × MVarId) := do
+      let type := if left then leftType else rightType
+      let newHypType ← mkForallFVars binderFVars type
+      let newHypProof ← mkLambdaFVars binderFVars $
+        mkAppN eliminator #[leftType, rightType, hypWithBinderFVars]
+      let goal ← assert goal originalUserName newHypType newHypProof
+      let (newHyp, goal) ← intro1 goal
+      return (newHyp, goal)
+
+    splitProduct (goal : MVarId)
+        (leftEliminator rightEliminator leftType rightType : Expr) :
+        MetaM (Array FVarId × MVarId) := do
+      let (leftHyp, goal) ←
+        splitProductHalf goal true  leftEliminator  leftType rightType
+      let (rightHyp, goal) ←
+        splitProductHalf goal false rightEliminator leftType rightType
+      let (goal, cleared) :=
+        match (← observing? $ clear goal hyp) with
+        | none => (goal, false)
+        | some goal => (goal, true)
+      let (leftHyps, goal)  ←
+        splitHypCore goal originalUserName binderFVars leftHyp  leftType
+      let (rightHyps, goal) ←
+        splitHypCore goal originalUserName binderFVars rightHyp rightType
+      let newHyps := (if cleared then #[] else #[hyp]) ++ leftHyps ++ rightHyps
+      return (newHyps, goal)
+
+    splitExistential (oldGoal : MVarId)
+        (witnessProjection propertyProjection witnessType propertyType : Expr) :
+        MetaM (Array FVarId × MVarId) := do
+
+      checkNotAssigned goal `splitHyp
+      let tag ← getMVarTag goal
+      let oldTarget ← getMVarType goal
+
+      -- I don't see how to make `assert` work with successive dependent
+      -- hypotheses, so here's a reimplementation. We assert one hypothesis for
+      -- the witness and one for the property, where the property hypothesis
+      -- depends on the witness hypothesis.
+      let witnessHypType ← mkForallFVars binderFVars witnessType
+      let newTarget ← do
+        withLocalDeclD originalUserName witnessHypType λ witness => do
+          let propertyHypType ←
+            mkForallFVars binderFVars $
+            (← headBeta (mkApp propertyType (mkAppN witness binderFVars)))
+          withLocalDeclD originalUserName propertyHypType λ property =>
+            mkForallFVars (#[witness, property]) oldTarget
+      let goal ← withMVarContext goal $
+        mkFreshExprSyntheticOpaqueMVar newTarget tag
+
+      let witnessHypProof ← mkLambdaFVars binderFVars $
+        mkAppN witnessProjection #[witnessType, propertyType, hypWithBinderFVars]
+      let propertyHypProof ← mkLambdaFVars binderFVars $
+        mkAppN propertyProjection #[witnessType, propertyType, hypWithBinderFVars]
+      let proof := mkAppN goal #[witnessHypProof, propertyHypProof]
+      assignExprMVar oldGoal proof
+
+      let goal := goal.mvarId!
+      let (#[witnessHyp, propertyHyp], goal) ← introN goal 2 | unreachable!
+
+      let (goal, cleared) :=
+        match (← observing? $ clear goal hyp) with
+        | none => (goal, false)
+        | some goal => (goal, true)
+      let propertyHypTypeWithoutBinders ←
+        headBeta (mkApp propertyType $ mkAppN (mkFVar witnessHyp) binderFVars)
+      let (newHyps, goal) ←
+        splitHypCore goal originalUserName binderFVars propertyHyp
+          propertyHypTypeWithoutBinders
+      let newHyps := (if cleared then #[] else #[hyp]) ++ newHyps
+      return (newHyps, goal)
+
+def splitHyp (goal : MVarId) (hyp : FVarId) : MetaM (Array FVarId × MVarId) :=
+  withMVarContext goal do
+    let decl ← getLocalDecl hyp
+    splitHypCore goal decl.userName #[] hyp decl.type
+
+def splitAllHyps (goal : MVarId) : MetaM (Array FVarId × MVarId) := do
+  let lctx := (← getMVarDecl goal).lctx
+  let mut goal := goal
+  let mut newHyps := #[]
+  for hyp in lctx do
+    if hyp.isAuxDecl then continue
+    let (newHyps', goal') ← splitHyp goal hyp.fvarId
+    newHyps := newHyps ++ newHyps'
+    goal := goal'
+  return (newHyps, goal)
+
+end Aesop.DefaultRules
