Aesop/Main.lean
@@ -1,0 +1,26 @@
+/-
+Copyright (c) 2021 Jannis Limperg. All rights reserved.
+Released under Apache 2.0 license as described in the file LICENSE.
+Authors: Jannis Limperg
+-/
+
+import Aesop.BestFirstSearch
+import Aesop.Config
+import Aesop.DefaultRules
+import Lean.Elab.Tactic
+
+namespace Aesop
+
+open Lean.Elab.Tactic
+
+@[tactic Parser.Tactic.aesop]
+def evalAesop : Tactic := λ stx =>
+  withMainContext do
+    let config ← TacticConfig.parse stx
+    let rs ← getRuleSet
+    let rs := rs.addArray (← defaultRules)
+    let rs := rs.addArray (← config.additionalRuleSetMembers)
+    trace[Aesop.RuleSet] m!"{rs}"
+    searchTactic rs
+
+end Aesop
