Aesop/RuleTac.lean
@@ -1,0 +1,84 @@
+/-
+Copyright (c) 2021 Jannis Limperg. All rights reserved.
+Released under Apache 2.0 license as described in the file LICENSE.
+Authors: Jannis Limperg
+-/
+
+import Lean.Elab
+
+open Lean
+open Lean.Elab.Tactic
+open Lean.Meta
+
+namespace Aesop
+
+-- A `RuleTacDescr` is a 'recipe' for constructing the tactic used by a rule.
+-- When we serialise the rule set to an olean file, we serialise `RuleTacDescr`s
+-- because we can't (currently?) serialise the actual tactics.
+inductive RuleTacDescr
+  | applyConst (decl : Name)
+  | tactic (decl : Name)
+  deriving Inhabited, BEq
+
+-- A `RuleTac` bundles a `RuleTacDescr` and the tactic that was computed from
+-- the description. Local rules do not have descriptions since we never
+-- serialise them.
+structure RuleTac where
+  tac : TacticM Unit
+  descr : Option RuleTacDescr
+  deriving Inhabited
+
+namespace RuleTacBuilder
+
+/- Convenience for evalTacticUnsafe. -/
+private abbrev TacticType := TacticM Unit
+
+def checkTacticM (decl : Name) : MetaM Unit := do
+  let info ← getConstInfo decl
+  unless (← isDefEq info.type (mkConst ``TacticType)) do
+    throwError "aesop: {decl} was expected to have type\n  TacticM Unit\nbut has type\n  {info.type}"
+
+unsafe def evalTacticConstUnsafe (decl : Name) : TacticM Unit := do
+  checkTacticM decl
+    -- TODO Maybe we can elide the above check. We already check the type
+    -- when we register the tactic.
+  let tac ← evalConst TacticType decl
+  tac
+
+@[implementedBy evalTacticConstUnsafe]
+constant evalTacticConst : Name → TacticM Unit
+-- I think the above use of `evalConst` is safe because we call it at a concrete
+-- type, making sure that the constant actually has that type.
+
+def tactic (decl : Name) : MetaM RuleTac := do
+  checkTacticM decl
+  return { tac := evalTacticConst decl, descr := RuleTacDescr.tactic decl }
+
+def apply (decl : Name) : MetaM RuleTac :=
+  return {
+    tac := liftMetaTactic λ goal => do
+      Lean.Meta.apply goal (← mkConstWithFreshMVarLevels decl)
+      -- TODO Go via apply tactic syntax to ensure intuitive behaviour?
+    descr := RuleTacDescr.applyConst decl
+  }
+
+def applyFVar (userName : Name) : MetaM RuleTac := do
+  let _ ← getLocalDeclFromUserName userName
+  return {
+    tac := liftMetaTactic λ goal => do
+      let decl ← getLocalDeclFromUserName userName
+      Lean.Meta.apply goal (mkFVar decl.fvarId)
+    descr := none
+  }
+
+end RuleTacBuilder
+
+namespace RuleTacDescr
+
+def toRuleTac : RuleTacDescr → MetaM RuleTac
+  | applyConst decl => RuleTacBuilder.apply decl
+  | tactic decl => RuleTacBuilder.tactic decl
+
+end RuleTacDescr
+
+end Aesop
