Aesop/Tracing.lean
@@ -1,0 +1,77 @@
+/-
+Copyright (c) 2021 Jannis Limperg. All rights reserved.
+Released under Apache 2.0 license as described in the file LICENSE.
+Authors: Jannis Limperg
+-/
+
+-- TODO Instead of tracing, I think we want to construct a couple of big
+-- messages at the end: one with the ruleset, one with the final search tree,
+-- one with the steps taken (displayed in a nice structured manner and hopefully
+-- inspectable).
+
+import Lean.Util.Trace
+
+open Lean
+
+-- TODO This block currently has no effect since `registerTraceClass` only
+-- works with builtin_initialize.
+initialize
+  registerTraceClass `Aesop.RuleSet
+  registerTraceClass `Aesop.Steps
+  registerTraceClass `Aesop.Steps.Goals
+  registerTraceClass `Aesop.Steps.UnsafeQueues
+  registerTraceClass `Aesop.Steps.FailedRuleApplications
+  registerTraceClass `Aesop.Steps.RuleSelection
+  registerTraceClass `Aesop.Steps.FinalProof
+  registerTraceClass `Aesop.Steps.Normalization
+  registerTraceClass `Aesop.Tree
+  registerTraceClass `Aesop.Tree.Goals
+  registerTraceClass `Aesop.Tree.UnsafeQueues
+  registerTraceClass `Aesop.Tree.FailedRuleApplications
+
+namespace Aesop
+
+inductive TraceContext
+  | steps
+  | tree
+
+namespace TraceContext
+
+@[inlineIfReduce]
+protected def toTraceOptionPrefix : TraceContext → Name
+  | steps => `trace.Aesop.Steps
+  | tree => `trace.Aesop.Tree
+
+end TraceContext
+
+inductive TraceOption : TraceContext → Type
+  | showGoals : TraceOption c
+  | showUnsafeQueues : TraceOption c
+  | showFailedRapps : TraceOption c
+  | showRuleSelection : TraceOption TraceContext.steps
+  | showFinalProof : TraceOption TraceContext.steps
+  | showNormalizationSteps : TraceOption TraceContext.steps
+
+namespace TraceOption
+
+@[inlineIfReduce]
+protected def toTraceOptionSuffix {c} : TraceOption c → Name
+  | showGoals => `Goals
+  | showUnsafeQueues => `UnsafeQueues
+  | showFailedRapps => `FailedRuleApplications
+  | showRuleSelection => `RuleSelection
+  | showFinalProof => `FinalProof
+  | showNormalizationSteps => `Normalization
+
+@[inline]
+protected def default {c} : TraceOption c → Bool :=
+  λ _ => true
+
+@[inline]
+def get [Monad m] [MonadOptions m] (c : TraceContext) (o : TraceOption c) :
+    m Bool :=
+  getBoolOption (c.toTraceOptionPrefix ++ o.toTraceOptionSuffix) o.default
+
+end TraceOption
+
+end Aesop
