Aesop/Util.lean
@@ -4,146 +4,27 @@ Released under Apache 2.0 license as described in the file LICENSE.
 Authors: Jannis Limperg, Asta Halkjær From
 -/
 
-import Lean
+import Aesop.Util.SudoSetOption
+import Lean.Elab.Syntax
+import Lean.Elab.Tactic.Basic
+import Lean.Message
+import Lean.Meta.DiscrTree
+import Lean.Meta.Tactic.Simp.SimpLemmas
+import Lean.Syntax
 import Std.Data.BinomialHeap
 
--- TODO remove
-def as (α : Type _) (a : α) : α := a
+namespace String
 
-notation : min a "@" T => as T a
+def joinSep (sep : String)  : List String → String
+  | [] => ""
+  | "" :: ss => joinSep sep ss
+  | s :: ss =>
+    let tail := joinSep sep ss
+    match tail with
+    | "" => s
+    | _ => s ++ sep ++ tail
 
-namespace List
-
-def findAndRemove (P : α → Prop) [DecidablePred P] : List α → Option (α × List α)
-  | [] => none
-  | (a :: as) =>
-    if P a
-      then some (a, as)
-      else
-        match findAndRemove P as with
-        | some (x, as) => some (x, a :: as)
-        | none => none
-
-section minimumBy
-
-variable (lt : α → α → Prop) [DecidableRel lt]
-
-def minimumBy₁ (a : α) (as : List α) : α :=
-  as.foldl (λ a a' => if lt a' a then a' else a) a
-
-def minimumBy : List α → Option α
-  | [] => none
-  | (a :: as) => some $ minimumBy₁ lt a as
-
-end minimumBy
-
-def minimum' [LT α] [DecidableRel (α := α) (· < ·)] : List α → Option α :=
-  minimumBy (· < ·)
-
-def minimum₁ [LT α] [DecidableRel (α := α) (· < ·)] : α → List α → α :=
-  minimumBy₁ (· < ·)
-
-end List
-
-
-namespace Std.PersistentHashSet
-
-@[inline]
-def merge [BEq α] [Hashable α] (s t : PersistentHashSet α) : PersistentHashSet α :=
-  if s.size < t.size then loop s t else loop t s
-  where
-    @[inline]
-    loop s t := s.fold (init := t) λ s a => s.insert a
-
-end Std.PersistentHashSet
-
-
-namespace Std.PersistentHashMap
-
-@[inline]
-def merge [BEq α] [Hashable α] (m n : PersistentHashMap α β) (f : α → β → β → β) :
-    PersistentHashMap α β :=
-  if m.size < n.size then loop m n f else loop n m (λ a b b' => f a b' b)
-  where
-    @[inline]
-    loop m n f := m.foldl (init := n) λ map k v =>
-      match map.find? k with
-      | some v' => map.insert k (f k v v')
-      | none => map.insert k v
-
-end Std.PersistentHashMap
-
-
-namespace Lean.Meta
-
--- TODO unused?
-def conclusionHeadConstant? (e : Expr) : MetaM (Option Name) :=
-  forallTelescope e $ λ _ e => e.getAppFn.constName?
-
-def copyMVar (mvarId : MVarId) : MetaM MVarId := do
-  let decl ← getMVarDecl mvarId
-  let mv ← mkFreshExprMVarAt decl.lctx decl.localInstances decl.type decl.kind
-    decl.userName decl.numScopeArgs
-  return mv.mvarId!
-
-namespace DiscrTree.Trie
-
-unsafe def foldMUnsafe [Monad m] (initialKeys : Array Key)
-    (f : σ → Array Key → α → m σ) (init : σ) : Trie α → m σ
-  | Trie.node vs children => do
-    let s ← vs.foldlM (init := init) λ s v => f s initialKeys v
-    children.foldlM (init := s) λ s (k, t) =>
-      t.foldMUnsafe (initialKeys.push k) f s
-
-@[implementedBy foldMUnsafe]
-constant foldM [Monad m] (initalKeys : Array Key)
-    (f : σ → Array Key → α → m σ) (init : σ) (t : Trie α) : m σ :=
-  pure init
-
-@[inline]
-def fold (initialKeys : Array Key) (f : σ → Array Key → α → σ) (init : σ)
-    (t : Trie α) : σ :=
-  Id.run $ foldM initialKeys (λ s k a => return f s k a) init t
-
-end Trie
-
-@[inline]
-def foldM [Monad m] (f : σ → Array Key → α → m σ) (init : σ) (t : DiscrTree α) :
-    m σ :=
-  t.root.foldlM (init := init) λ s k t => t.foldM #[k] (init := s) f
-
-@[inline]
-def fold (f : σ → Array Key → α → σ) (init : σ) (t : DiscrTree α) : σ :=
-  Id.run $ foldM (λ s keys a => return f s keys a) init t
-
--- TODO inefficient since it doesn't take advantage of the Trie structure at all
-@[inline]
-def merge [BEq α] (t u : DiscrTree α) : DiscrTree α :=
-  if t.root.size < u.root.size then loop t u else loop u t
-  where
-    loop t u := t.fold (init := u) λ u keys a => DiscrTree.insertCore u keys a
-
-end DiscrTree
-
-namespace SimpLemmas
-
-def empty : SimpLemmas where
-  pre := DiscrTree.mk (Std.PersistentHashMap.empty)
-  post := DiscrTree.mk (Std.PersistentHashMap.empty)
-  lemmaNames := Std.PersistentHashSet.empty
-  toUnfold := Std.PersistentHashSet.empty
-  erased := Std.PersistentHashSet.empty
-
-def merge (s t : SimpLemmas) : SimpLemmas where
-  pre := s.pre.merge t.pre
-  post := s.post.merge t.post
-  lemmaNames := s.lemmaNames.merge t.lemmaNames
-  toUnfold := s.toUnfold.merge t.toUnfold
-  erased := s.erased.merge t.erased
-
-end SimpLemmas
-
-end Lean.Meta
+end String
 
 
 namespace Std.Format
@@ -155,20 +36,21 @@ def isEmptyShallow : Format → Bool
   | _ => false
 
 @[inline]
-def indentDSkipEmpty (f : Format) : Format :=
+def indentDSkipEmpty [ToFormat α] (f : α) : Format :=
+  let f := format f
   if f.isEmptyShallow then nil else indentD f
 
 @[inline]
-def unlines (fs : List Format) : Format :=
+def unlines [ToFormat α] (fs : List α) : Format :=
   Format.joinSep fs line
 
 @[inline]
-def indentDUnlines : List Format → Format :=
+def indentDUnlines [ToFormat α] : List α → Format :=
   indentDSkipEmpty ∘ unlines
 
 @[inline]
-def indentDUnlinesSkipEmpty (fs : List Format) : Format :=
-  indentDSkipEmpty $ unlines $ fs.filter (¬ ·.isEmptyShallow)
+def indentDUnlinesSkipEmpty [ToFormat α] (fs : List α) : Format :=
+  indentDSkipEmpty $ unlines (fs.map format |>.filter (¬ ·.isEmptyShallow))
 
 def formatIf (b : Bool) (f : Thunk Format) : Format :=
   if b then f.get else nil
@@ -206,7 +88,285 @@ def indentDUnlinesSkipEmpty (fs : List MessageData) : MessageData :=
 def toMessageDataIf (b : Bool) (f : Thunk MessageData) : MessageData :=
   if b then f.get else nil
 
+def nodeFiltering (fs : Array (Option MessageData)) : MessageData :=
+  node $ fs.filterMap id
+
 end Lean.MessageData
+
+
+namespace Std.PersistentHashSet
+
+@[inline]
+def merge [BEq α] [Hashable α] (s t : PersistentHashSet α) : PersistentHashSet α :=
+  if s.size < t.size then loop s t else loop t s
+  where
+    @[inline]
+    loop s t := s.fold (init := t) λ s a => s.insert a
+
+-- Elements are returned in unspecified order.
+def toList [BEq α] [Hashable α] (s : PersistentHashSet α) : List α :=
+  s.fold (init := []) λ as a => a :: as
+
+-- Elements are returned in unspecified order. (In fact, they are currently
+-- returned in reverse order of `toList`.)
+def toArray [BEq α] [Hashable α] (s : PersistentHashSet α) : Array α :=
+  s.fold (init := #[]) λ as a => as.push a
+
+end Std.PersistentHashSet
+
+
+namespace Std.PersistentHashMap
+
+@[inline]
+def merge [BEq α] [Hashable α] (m n : PersistentHashMap α β) (f : α → β → β → β) :
+    PersistentHashMap α β :=
+  if m.size < n.size then loop m n f else loop n m (λ a b b' => f a b' b)
+  where
+    @[inline]
+    loop m n f := m.foldl (init := n) λ map k v =>
+      match map.find? k with
+      | some v' => map.insert k (f k v v')
+      | none => map.insert k v
+
+universe u v
+
+-- We need to give u and v explicitly here, otherwise the compiler gets
+-- confused.
+unsafe def forInImpl [BEq α] [Hashable α] {m : Type u → Type v} [Monad m]
+    (map : PersistentHashMap α β) (init : σ) (f : α × β → σ → m (ForInStep σ)) :
+    m σ := do
+  match (← go map.root init) with
+  | ForInStep.yield r => pure r
+  | ForInStep.done r => pure r
+  where
+    go : Node α β → σ → m (ForInStep σ)
+      | Node.collision keys vals heq, acc =>
+        let rec go' (i : Nat) (acc : σ) : m (ForInStep σ) := do
+          if h : i < keys.size then
+            let k := keys.get ⟨i, h⟩
+            let v := vals.get ⟨i, heq ▸ h⟩
+            match (← f (k, v) acc) with
+            | ForInStep.done result => return ForInStep.done result
+            | ForInStep.yield acc => go' (i + 1) acc
+          else
+            return ForInStep.yield acc
+        go' 0 acc
+      | Node.entries entries, acc => do
+        let mut acc := acc
+        for entry in entries do
+          match entry with
+          | Entry.null => pure ⟨⟩
+          | Entry.entry k v =>
+            match (← f (k, v) acc) with
+            | ForInStep.done result => return ForInStep.done result
+            | ForInStep.yield acc' => acc := acc'
+          | Entry.ref node =>
+            match (← go node acc) with
+            | ForInStep.done result => return ForInStep.done result
+            | ForInStep.yield acc' => acc := acc'
+        return ForInStep.yield acc
+
+-- Inhabited inference is being stupid here, so we can't use `partial`.
+@[implementedBy forInImpl]
+constant forIn [BEq α] [Hashable α] {m : Type u → Type v} [Monad m]
+  (map : PersistentHashMap α β) (init : σ) (f : α × β → σ → m (ForInStep σ)) :
+  m σ :=
+  pure init
+
+instance [BEq α] [Hashable α] : ForIn m (PersistentHashMap α β) (α × β) where
+  forIn map := map.forIn
+
+end Std.PersistentHashMap
+
+
+namespace Lean.Meta.DiscrTree.Trie
+
+unsafe def foldMUnsafe [Monad m] (initialKeys : Array Key)
+    (f : σ → Array Key → α → m σ) (init : σ) : Trie α → m σ
+  | Trie.node vs children => do
+    let s ← vs.foldlM (init := init) λ s v => f s initialKeys v
+    children.foldlM (init := s) λ s (k, t) =>
+      t.foldMUnsafe (initialKeys.push k) f s
+
+@[implementedBy foldMUnsafe]
+constant foldM [Monad m] (initalKeys : Array Key)
+    (f : σ → Array Key → α → m σ) (init : σ) (t : Trie α) : m σ :=
+  pure init
+
+@[inline]
+def fold (initialKeys : Array Key) (f : σ → Array Key → α → σ) (init : σ)
+    (t : Trie α) : σ :=
+  Id.run $ t.foldM initialKeys (init := init) λ s k a => return f s k a
+
+end Trie
+
+@[inline]
+def foldM [Monad m] (f : σ → Array Key → α → m σ) (init : σ) (t : DiscrTree α) :
+    m σ :=
+  t.root.foldlM (init := init) λ s k t => t.foldM #[k] (init := s) f
+
+@[inline]
+def fold (f : σ → Array Key → α → σ) (init : σ) (t : DiscrTree α) : σ :=
+  Id.run $ t.foldM (init := init) λ s keys a => return f s keys a
+
+-- TODO inefficient since it doesn't take advantage of the Trie structure at all
+@[inline]
+def merge [BEq α] (t u : DiscrTree α) : DiscrTree α :=
+  if t.root.size < u.root.size then loop t u else loop u t
+  where
+    @[inline]
+    loop t u := t.fold (init := u) DiscrTree.insertCore
+
+def values (t : DiscrTree α) : Array α :=
+  t.fold (init := #[]) λ as _ a => as.push a
+
+def toArray (t : DiscrTree α) : Array (Array Key × α) :=
+  t.fold (init := #[]) λ as keys a => as.push (keys, a)
+
+end DiscrTree
+
+
+namespace SimpLemmas
+
+def merge (s t : SimpLemmas) : SimpLemmas where
+  pre := s.pre.merge t.pre
+  post := s.post.merge t.post
+  lemmaNames := s.lemmaNames.merge t.lemmaNames
+  toUnfold := s.toUnfold.merge t.toUnfold
+  erased := s.erased.merge t.erased
+
+def addSimpEntry (s : SimpLemmas) : SimpEntry → SimpLemmas
+  | SimpEntry.lemma l => addSimpLemmaEntry s l
+  | SimpEntry.toUnfold d => s.addDeclToUnfold d
+
+open MessageData in
+protected def toMessageData (s : SimpLemmas) : MessageData :=
+  node #[
+    "pre lemmas:" ++ node (s.pre.values.map toMessageData),
+    "post lemmas:" ++ node (s.post.values.map toMessageData),
+    "definitions to unfold:" ++ node
+      (s.toUnfold.toArray.qsort Name.lt |>.map toMessageData),
+    "erased entries:" ++ node
+      (s.erased.toArray.qsort Name.lt |>.map toMessageData)
+  ]
+
+end SimpLemmas
+
+-- TODO The following defs are copied from Lean.Meta.Tactic.Simp.SimpLemmas
+
+private partial def shouldPreprocess (type : Expr) : MetaM Bool :=
+  forallTelescopeReducing type fun xs result => return !result.isEq
+
+private def checkTypeIsProp (type : Expr) : MetaM Unit :=
+  unless (← isProp type) do
+    throwError "invalid 'simp', proposition expected{indentExpr type}"
+
+private partial def isPerm : Expr → Expr → MetaM Bool
+  | Expr.app f₁ a₁ _, Expr.app f₂ a₂ _ => isPerm f₁ f₂ <&&> isPerm a₁ a₂
+  | Expr.mdata _ s _, t => isPerm s t
+  | s, Expr.mdata _ t _ => isPerm s t
+  | s@(Expr.mvar ..), t@(Expr.mvar ..) => isDefEq s t
+  | Expr.forallE n₁ d₁ b₁ _, Expr.forallE n₂ d₂ b₂ _ => isPerm d₁ d₂ <&&> withLocalDeclD n₁ d₁ fun x => isPerm (b₁.instantiate1 x) (b₂.instantiate1 x)
+  | Expr.lam n₁ d₁ b₁ _, Expr.lam n₂ d₂ b₂ _ => isPerm d₁ d₂ <&&> withLocalDeclD n₁ d₁ fun x => isPerm (b₁.instantiate1 x) (b₂.instantiate1 x)
+  | Expr.letE n₁ t₁ v₁ b₁ _, Expr.letE n₂ t₂ v₂ b₂ _ =>
+    isPerm t₁ t₂ <&&> isPerm v₁ v₂ <&&> withLetDecl n₁ t₁ v₁ fun x => isPerm (b₁.instantiate1 x) (b₂.instantiate1 x)
+  | Expr.proj _ i₁ b₁ _, Expr.proj _ i₂ b₂ _ => i₁ == i₂ <&&> isPerm b₁ b₂
+  | s, t => s == t
+
+private partial def preprocess (e type : Expr) : MetaM (List (Expr × Expr)) := do
+  let type ← whnf type
+  if type.isForall then
+    forallTelescopeReducing type fun xs type => do
+      let e := mkAppN e xs
+      let ps ← preprocess e type
+      ps.mapM fun (e, type) =>
+        return (← mkLambdaFVars xs e, ← mkForallFVars xs type)
+  else if type.isEq then
+    return [(e, type)]
+  else if let some (lhs, rhs) := type.iff? then
+    let type ← mkEq lhs rhs
+    let e    ← mkPropExt e
+    return [(e, type)]
+  else if let some (_, lhs, rhs) := type.ne? then
+    let type ← mkEq (← mkEq lhs rhs) (mkConst ``False)
+    let e    ← mkEqFalse e
+    return [(e, type)]
+  else if let some p := type.not? then
+    let type ← mkEq p (mkConst ``False)
+    let e    ← mkEqFalse e
+    return [(e, type)]
+  else if let some (type₁, type₂) := type.and? then
+    let e₁ := mkProj ``And 0 e
+    let e₂ := mkProj ``And 1 e
+    return (← preprocess e₁ type₁) ++ (← preprocess e₂ type₂)
+  else
+    let type ← mkEq type (mkConst ``True)
+    let e    ← mkEqTrue e
+    return [(e, type)]
+
+private def mkSimpLemmaCore (e : Expr) (levelParams : Array Name) (proof : Expr) (post : Bool) (prio : Nat) (name? : Option Name) : MetaM SimpLemma := do
+  let type ← instantiateMVars (← inferType e)
+  withNewMCtxDepth do
+    let (xs, _, type) ← withReducible <| forallMetaTelescopeReducing type
+    let type ← whnfR type
+    let (keys, perm) ←
+      match type.eq? with
+      | some (_, lhs, rhs) => pure (← DiscrTree.mkPath lhs, ← isPerm lhs rhs)
+      | none => throwError "unexpected kind of 'simp' theorem{indentExpr type}"
+    return { keys := keys, perm := perm, post := post, levelParams := levelParams, proof := proof, name? := name?, priority := prio }
+
+def mkSimpLemmasFromConst (declName : Name) (post : Bool) (prio : Nat) : MetaM (Array SimpLemma) := do
+  let cinfo ← getConstInfo declName
+  let val := mkConst declName (cinfo.levelParams.map mkLevelParam)
+  withReducible do
+    let type ← inferType val
+    checkTypeIsProp type
+    if (← shouldPreprocess type) then
+      let mut r := #[]
+      for (val, type) in (← preprocess val type) do
+        let auxName ← mkAuxLemma cinfo.levelParams type val
+        r := r.push <| (← mkSimpLemmaCore (mkConst auxName (cinfo.levelParams.map mkLevelParam)) #[] (mkConst auxName) post prio declName)
+      return r
+    else
+      #[← mkSimpLemmaCore (mkConst declName (cinfo.levelParams.map mkLevelParam)) #[] (mkConst declName) post prio declName]
+
+def copyMVar (mvarId : MVarId) : MetaM MVarId := do
+  let decl ← getMVarDecl mvarId
+  let mv ← mkFreshExprMVarAt decl.lctx decl.localInstances decl.type decl.kind
+    decl.userName decl.numScopeArgs
+  return mv.mvarId!
+
+end Lean.Meta
+
+
+namespace Std.BinomialHeap
+
+@[inline]
+def removeMin {lt : α → α → Bool} (h : BinomialHeap α lt) :
+    Option (α × BinomialHeap α lt) :=
+  match h.head? with
+  | some hd => some (hd, h.tail)
+  | none => none
+
+end Std.BinomialHeap
+
+
+namespace MonadStateOf
+
+@[inline]
+def ofLens [Monad m] [MonadStateOf α m] (project : α → β) (inject : β → α → α) :
+    MonadStateOf β m where
+  get := return project (← get)
+  set b := modify λ a => inject b a
+  modifyGet f := modifyGet λ a =>
+    let (r, b) := f (project a)
+    (r, inject b a)
+
+end MonadStateOf
+
+@[inline]
+abbrev setThe (σ) {m} [MonadStateOf σ m] (s : σ) : m PUnit :=
+  MonadStateOf.set s
 
 
 namespace ST.Ref
@@ -240,31 +400,131 @@ def modifyGetM (r : Ref σ α) (f : α → m (β × α)) : m β := do
 end ST.Ref
 
 
-namespace Std.BinomialHeap
+namespace Lean.Meta
 
-@[inline]
-def removeMin {lt : α → α → Bool} (h : BinomialHeap α lt) :
-    Option (α × BinomialHeap α lt) :=
-  match h.head? with
-  | some hd => some (hd, h.tail)
-  | none => none
+def instantiateMVarsMVarType (mvarId : MVarId) : MetaM Expr := do
+  let type ← instantiateMVars (← getMVarDecl mvarId).type
+  setMVarType mvarId type
+  return type
 
-end Std.BinomialHeap
+end Lean.Meta
 
 
-namespace MonadStateOf
+namespace Lean.Syntax
 
-@[inline]
-def ofLens [Monad m] [MonadStateOf α m] (project : α → β) (inject : β → α → α) :
-    MonadStateOf β m where
-  get := return project (← get)
-  set b := modify λ a => inject b a
-  modifyGet f := modifyGet λ a =>
-    let (r, b) := f (project a)
-    (r, inject b a)
+-- TODO for debugging, maybe remove
+partial def formatRaw : Syntax → String
+  | missing => "missing"
+  | node kind args =>
+    let args := ", ".joinSep $ args.map formatRaw |>.toList
+    s!"(node {kind} [{args}])"
+  | atom _ val => s!"(atom {val})"
+  | ident _ _ val _ => s!"(ident {val})"
 
-end MonadStateOf
+end Lean.Syntax
 
-@[inline]
-abbrev setThe (σ) {m} [MonadStateOf σ m] (s : σ) : m PUnit :=
-  MonadStateOf.set s
+
+namespace Lean
+
+open Lean.Elab.Tactic
+
+def runTacticMAsMetaM (tac : TacticM Unit) (goal : MVarId) :
+    MetaM (List MVarId) :=
+  run goal tac |>.run'
+
+def runMetaMAsImportM (x : MetaM α) : ImportM α := do
+  let ctx : Core.Context := { options := (← read).opts }
+  let state : Core.State := { env := (← read).env }
+  let r ← x |>.run {} {} |>.run ctx state |>.toIO'
+  match r with
+  | Except.ok ((a, _), _) => pure a
+  | Except.error e => throw $ IO.userError (← e.toMessageData.toString)
+
+def runMetaMAsCoreM (x : MetaM α) : CoreM α :=
+  Prod.fst <$> x.run {} {}
+
+end Lean
+
+
+namespace Lean.Elab.Command
+
+syntax (name := syntaxCatWithUnreservedTokens)
+  "declare_syntax_cat' " ident
+    (&"allow_leading_unreserved_tokens" <|> &"force_leading_unreserved_tokens")? : command
+
+-- Copied from Lean/Elab/Syntax.lean
+private def declareSyntaxCatQuotParser (catName : Name) : CommandElabM Unit := do
+  if let Name.str _ suffix _ := catName then
+    let quotSymbol := "`(" ++ suffix ++ "|"
+    let name := catName ++ `quot
+    -- TODO(Sebastian): this might confuse the pretty printer, but it lets us reuse the elaborator
+    let kind := ``Lean.Parser.Term.quot
+    let cmd ← `(
+      @[termParser] def $(mkIdent name) : Lean.ParserDescr :=
+        Lean.ParserDescr.node $(quote kind) $(quote Lean.Parser.maxPrec)
+          (Lean.ParserDescr.binary `andthen (Lean.ParserDescr.symbol $(quote quotSymbol))
+            (Lean.ParserDescr.binary `andthen
+              (Lean.ParserDescr.unary `incQuotDepth (Lean.ParserDescr.cat $(quote catName) 0))
+              (Lean.ParserDescr.symbol ")"))))
+    elabCommand cmd
+
+open Lean.Parser (LeadingIdentBehavior) in
+@[commandElab syntaxCatWithUnreservedTokens]
+def elabDeclareSyntaxCatWithUnreservedTokens : CommandElab := fun stx => do
+  let catName  := stx[1].getId
+  let leadingIdentBehavior :=
+    match stx[2].getOptional? with
+    | none => LeadingIdentBehavior.default
+    | some b =>
+      match b.getAtomVal! with
+      | "allow_leading_unreserved_tokens" => LeadingIdentBehavior.both
+      | "force_leading_unreserved_tokens" => LeadingIdentBehavior.symbol
+      | _ => unreachable!
+  let attrName := catName.appendAfter "Parser"
+  let env ← getEnv
+  let env ←
+    liftIO $ Parser.registerParserCategory env attrName catName
+      leadingIdentBehavior
+  setEnv env
+  declareSyntaxCatQuotParser catName
+
+end Lean.Elab.Command
+
+
+namespace Lean.Elab.Tactic
+
+open Lean.Elab.Term
+open Lean.Meta
+
+syntax (name := Parser.runTactic) &"run" term : tactic
+
+private abbrev TacticMUnit := TacticM Unit
+
+-- TODO copied from evalExpr
+unsafe def evalTacticMUnitUnsafe (value : Expr) : TermElabM (TacticM Unit) :=
+  withoutModifyingEnv do
+    let name ← mkFreshUserName `_tmp
+    let type ← inferType value
+    unless (← isDefEq type (mkConst ``TacticMUnit)) do
+      throwError "unexpected type at evalTacticMUnit:{indentExpr type}"
+    let decl := Declaration.defnDecl {
+       name := name, levelParams := [], type := type,
+       value := value, hints := ReducibilityHints.opaque,
+       safety := DefinitionSafety.unsafe
+    }
+    ensureNoUnassignedMVars decl
+    addAndCompile decl
+    evalConst (TacticM Unit) name
+
+@[implementedBy evalTacticMUnitUnsafe]
+constant evalTacticMUnit : Expr → TermElabM (TacticM Unit)
+
+@[tactic Parser.runTactic]
+def evalRunTactic : Tactic
+  | `(tactic|run $t:term) => do
+    let t ← elabTerm t (some (mkApp (mkConst ``TacticM) (mkConst ``Unit)))
+    let t ← evalTacticMUnit t
+    t
+  | _ => unreachable!
+
+end Lean.Elab.Tactic
