tests/Aesop.lean
@@ -1,0 +1,44 @@
+/-
+Copyright (c) 2021 Jannis Limperg. All rights reserved.
+Released under Apache 2.0 license as described in the file LICENSE.
+Authors: Jannis Limperg
+-/
+
+-- TODO clean up this test case
+import Lean
+import Aesop.Main
+
+open Lean
+open Lean.Meta
+open Lean.Elab.Tactic
+
+inductive Even : Nat → Prop
+| zero : Even Nat.zero
+| plus_two {n} : Even n → Even (Nat.succ (Nat.succ n))
+
+inductive Odd : Nat → Prop
+| one : Odd (Nat.succ Nat.zero)
+| plus_two {n} : Odd n → Odd (Nat.succ (Nat.succ n))
+
+inductive EvenOrOdd : Nat → Prop
+| even {n} : Even n → EvenOrOdd n
+| odd {n} : Odd n → EvenOrOdd n
+
+attribute [aesop  50%] EvenOrOdd.even EvenOrOdd.odd
+attribute [aesop safe] Even.zero Even.plus_two
+attribute [aesop 100%] Odd.one Odd.plus_two
+
+def EvenOrOdd' (n : Nat) : Prop := EvenOrOdd n
+
+@[aesop norm (builder tactic)]
+def testNormTactic : TacticM Unit := do
+  evalTactic (← `(tactic|try simp only [EvenOrOdd']))
+
+set_option pp.all false
+sudo set_option trace.Aesop.RuleSet false
+sudo set_option trace.Aesop.Steps false
+
+example : EvenOrOdd' 3 := by aesop
+
+-- In this example, the goal is solved already during normalisation.
+example : 0 = 0 := by aesop
