tests/Mathlib4.lean
@@ -1,0 +1,418 @@
+import Aesop.Main
+
+theorem EqIffBeqTrue [DecidableEq α] {a b : α} : a = b ↔ ((a == b) = true) :=
+⟨decideEqTrue, ofDecideEqTrue⟩
+
+theorem NeqIffBeqFalse [DecidableEq α] {a b : α} : a ≠ b ↔ ((a == b) = false) :=
+⟨decideEqFalse, ofDecideEqFalse⟩
+
+theorem decide_eq_true_iff (p : Prop) [Decidable p] : (decide p = true) ↔ p :=
+⟨ofDecideEqTrue, decideEqTrue⟩
+
+theorem decide_eq_false_iff_not (p : Prop) [Decidable p] : (decide p = false) ↔ ¬ p :=
+⟨ofDecideEqFalse, decideEqFalse⟩
+
+theorem optParam_eq (α : Sort u) (default : α) : optParam α default = α := rfl
+
+def not_false := notFalse
+def proof_irrel := @proofIrrel
+def congr_fun := @congrFun
+def congr_arg := @congrArg
+def of_eq_true := @ofEqTrue
+
+-- TODO subst builder
+theorem not_of_eq_false {p : Prop} (h : p = False) : ¬p := fun hp => h ▸ hp
+
+-- TODO reflexivity default tactic
+-- TODO How to use a lemma like this? Imo this is a nice example of e-matching.
+theorem cast_proof_irrel (h₁ h₂ : α = β) (a : α) : cast h₁ a = cast h₂ a := rfl
+
+def cast_eq := @castEq
+
+-- TODO make this a norm lemma?
+theorem Ne.def (a b : α) : (a ≠ b) = ¬ (a = b) := rfl
+
+def false_of_ne := @falseOfNe
+def ne_false_of_self := @neFalseOfSelf
+def ne_true_of_not := @neTrueOfNot
+def true_ne_false := trueNeFalse
+def eq_of_heq := @eqOfHEq
+def heq_of_eq := @heqOfEq
+def heq_of_heq_of_eq := @heqOfHEqOfEq
+def heq_of_eq_of_heq := @heqOfEqOfHEq
+def type_eq_of_heq := @typeEqOfHEq
+def eq_rec_heq := @eqRecHEq
+
+-- TODO heq refl default tactic
+theorem heq_of_eq_rec_left {φ : α → Sort v} {a a' : α} {p₁ : φ a} {p₂ : φ a'} :
+  (e : a = a') → (h₂ : Eq.rec (motive := fun a _ => φ a) p₁ e = p₂) → p₁ ≅ p₂
+| rfl, rfl => HEq.rfl
+
+theorem heq_of_eq_rec_right {φ : α → Sort v} {a a' : α} {p₁ : φ a} {p₂ : φ a'} :
+  (e : a' = a) → (h₂ : p₁ = Eq.rec (motive := fun a _ => φ a) p₂ e) → p₁ ≅ p₂
+| rfl, rfl => HEq.rfl
+
+theorem of_heq_true (h : a ≅ True) : a := of_eq_true (eq_of_heq h)
+
+def cast_heq := @castHEq
+
+-- TODO use applicable hyps by default
+def And.elim (f : a → b → α) (h : a ∧ b) : α := by aesop (safe [f])
+
+theorem And.symm : a ∧ b → b ∧ a := by aesop
+
+-- TODO automatic cases on or in hyp (needs per-hyp rules)
+-- TODO cases builder
+theorem Or.elim {a b c : Prop} (h₁ : a → c) (h₂ : b → c) (h : a ∨ b) : c := by
+  cases h <;> aesop
+
+-- TODO make normalisation a fixpoint loop?
+-- TODO deal with negation
+-- TODO use hyps in the context by default
+theorem not_not_em (a : Prop) : ¬¬(a ∨ ¬a) := by
+  show ((a ∨ (a → False)) → False) → False
+  exact fun H => H (Or.inr fun h => H (Or.inl h))
+
+theorem Or.symm (h : a ∨ b) : b ∨ a := by
+  cases h <;> aesop
+
+-- TODO use iff in the context as norm rule?
+-- TODO allow local hyps to be added as norm simp rules
+def Iff.elim (f : (a → b) → (b → a) → c) (h : a ↔ b) : c := by
+  admit
+  -- aesop (norm [h (builder simp)])
+
+-- TODO add Iff.intro as default rule
+theorem iff_comm : (a ↔ b) ↔ (b ↔ a) := by
+  aesop (safe [Iff.intro])
+
+theorem iff_iff_implies_and_implies : (a ↔ b) ↔ (a → b) ∧ (b → a) :=
+  ⟨fun ⟨ha, hb⟩ => ⟨ha, hb⟩, fun ⟨ha, hb⟩ => ⟨ha, hb⟩⟩
+
+-- TODO don't do contextual simp for all hyps by default (so this should fail)
+theorem Eq.to_iff : a = b → (a ↔ b) := by
+  aesop
+
+theorem neq_of_not_iff : ¬(a ↔ b) → a ≠ b := mt Eq.to_iff
+
+theorem of_iff_true (h : a ↔ True) : a := by aesop
+
+theorem not_of_iff_false : (a ↔ False) → ¬a := Iff.mp
+
+theorem not_not_intro : a → ¬¬a := fun a h => h a
+
+theorem iff_true_intro (h : a) : a ↔ True := by aesop
+
+theorem iff_false_intro (h : ¬a) : a ↔ False := by aesop
+
+theorem not_iff_false_intro (h : a) : ¬a ↔ False := by aesop
+
+theorem not_not_not : ¬¬¬a ↔ ¬a := ⟨mt not_not_intro, not_not_intro⟩
+
+theorem imp_congr_left (h : a ↔ b) : (a → c) ↔ (b → c) := by aesop
+
+-- TODO Iff elim
+theorem imp_congr_right (h : a → (b ↔ c)) : (a → b) ↔ (a → c) :=
+⟨fun hab ha => (h ha).1 (hab ha), fun hcd ha => (h ha).2 (hcd ha)⟩
+
+theorem imp_congr_ctx (h₁ : a ↔ c) (h₂ : c → (b ↔ d)) : (a → b) ↔ (c → d) :=
+(imp_congr_left h₁).trans (imp_congr_right h₂)
+
+theorem imp_congr (h₁ : a ↔ c) (h₂ : b ↔ d) : (a → b) ↔ (c → d) := by
+  aesop (safe [imp_congr_ctx])
+  -- imp_congr_ctx h₁ fun _ => h₂
+
+theorem Not.intro {a : Prop} (h : a → False) : ¬a := by aesop
+
+-- TODO try False-elim with low priority if we have a hyp X → False in the
+-- context.
+def Not.elim (h : ¬a) (ha : a) : α := by aesop
+
+theorem not_true : ¬True ↔ False := by aesop
+
+theorem not_false_iff : ¬False ↔ True := by aesop
+
+theorem not_congr (h : a ↔ b) : ¬a ↔ ¬b := by aesop
+
+theorem ne_self_iff_false (a : α) : a ≠ a ↔ False := by aesop
+
+theorem eq_self_iff_true (a : α) : a = a ↔ True := by aesop
+
+theorem heq_self_iff_true (a : α) : a ≅ a ↔ True := iff_true_intro HEq.rfl
+
+theorem iff_not_self : ¬(a ↔ ¬a) | H => let f h := H.1 h h; f (H.2 f)
+
+theorem not_iff_self : ¬(¬a ↔ a) | H => iff_not_self H.symm
+
+theorem eq_comm {a b : α} : a = b ↔ b = a := ⟨Eq.symm, Eq.symm⟩
+
+theorem And.imp (f : a → c) (g : b → d) (h : a ∧ b) : c ∧ d := ⟨f h.1, g h.2⟩
+
+theorem and_congr (h₁ : a ↔ c) (h₂ : b ↔ d) : a ∧ b ↔ c ∧ d := ⟨And.imp h₁.1 h₂.1, And.imp h₁.2 h₂.2⟩
+
+theorem and_congr_right (h : a → (b ↔ c)) : (a ∧ b) ↔ (a ∧ c) :=
+⟨fun ⟨ha, hb⟩ => ⟨ha, (h ha).1 hb⟩, fun ⟨ha, hb⟩ => ⟨ha, (h ha).2 hb⟩⟩
+
+theorem and_comm : a ∧ b ↔ b ∧ a := ⟨And.symm, And.symm⟩
+
+theorem and_assoc : (a ∧ b) ∧ c ↔ a ∧ (b ∧ c) :=
+⟨fun ⟨⟨ha, hb⟩, hc⟩ => ⟨ha, hb, hc⟩, fun ⟨ha, hb, hc⟩ => ⟨⟨ha, hb⟩, hc⟩⟩
+
+theorem and_left_comm : a ∧ (b ∧ c) ↔ b ∧ (a ∧ c) := by
+  rw [← and_assoc, ← and_assoc, @and_comm a b]
+  exact Iff.rfl
+
+theorem and_iff_left (hb : b) : a ∧ b ↔ a := ⟨And.left, fun ha => ⟨ha, hb⟩⟩
+
+theorem and_iff_right (ha : a) : a ∧ b ↔ b := ⟨And.right, fun hb => ⟨ha, hb⟩⟩
+
+theorem and_true : a ∧ True ↔ a := and_iff_left ⟨⟩
+
+theorem true_and : True ∧ a ↔ a := and_iff_right ⟨⟩
+
+theorem and_false : a ∧ False ↔ False := iff_false_intro And.right
+
+theorem false_and : False ∧ a ↔ False := iff_false_intro And.left
+
+theorem and_not_self : ¬(a ∧ ¬a) | ⟨ha, hn⟩ => hn ha
+theorem not_and_self : ¬(¬a ∧ a) | ⟨hn, ha⟩ => hn ha
+
+theorem and_self : a ∧ a ↔ a := ⟨And.left, fun h => ⟨h, h⟩⟩
+
+theorem Or.imp (f : a → c) (g : b → d) (h : a ∨ b) : c ∨ d := h.elim (inl ∘ f) (inr ∘ g)
+
+theorem Or.imp_left (f : a → b) : a ∨ c → b ∨ c := Or.imp f id
+
+theorem Or.imp_right (f : b → c) : a ∨ b → a ∨ c := Or.imp id f
+
+theorem or_congr (h₁ : a ↔ c) (h₂ : b ↔ d) : (a ∨ b) ↔ (c ∨ d) :=
+⟨Or.imp h₁.1 h₂.1, Or.imp h₁.2 h₂.2⟩
+
+theorem or_comm : a ∨ b ↔ b ∨ a := ⟨Or.symm, Or.symm⟩
+
+theorem Or.resolve_left (h : a ∨ b) (na : ¬a) : b := h.elim na.elim id
+
+theorem Or.neg_resolve_left (h : ¬a ∨ b) (ha : a) : b := h.elim (absurd ha) id
+
+theorem Or.resolve_right (h : a ∨ b) (nb : ¬b) : a := h.elim id nb.elim
+
+theorem Or.neg_resolve_right (h : a ∨ ¬b) (nb : b) : a := h.elim id (absurd nb)
+
+open Or in
+theorem or_assoc {a b c} : (a ∨ b) ∨ c ↔ a ∨ (b ∨ c) :=
+⟨fun | inl (inl h) => inl h
+     | inl (inr h) => inr (inl h)
+     | inr h => inr (inr h),
+ fun | inl h => inl (inl h)
+     | inr (inl h) => inl (inr h)
+     | inr (inr h) => inr h⟩
+
+theorem or_left_comm : a ∨ (b ∨ c) ↔ b ∨ (a ∨ c) := by
+  rw [← or_assoc, ← or_assoc, @or_comm a b]
+  exact Iff.rfl
+
+theorem or_true : a ∨ True ↔ True := iff_true_intro (Or.inr ⟨⟩)
+
+theorem true_or : True ∨ a ↔ True := iff_true_intro (Or.inl ⟨⟩)
+
+theorem or_false : a ∨ False ↔ a := ⟨fun h => h.resolve_right id, Or.inl⟩
+
+theorem false_or : False ∨ a ↔ a := ⟨fun h => h.resolve_left id, Or.inr⟩
+
+theorem or_self : a ∨ a ↔ a := ⟨fun h => h.elim id id, Or.inl⟩
+
+theorem not_or_intro : (na : ¬a) → (nb : ¬b) → ¬(a ∨ b) := Or.elim
+
+theorem not_or (p q) : ¬ (p ∨ q) ↔ ¬ p ∧ ¬ q :=
+⟨fun H => ⟨mt Or.inl H, mt Or.inr H⟩, fun ⟨hp, hq⟩ pq => pq.elim hp hq⟩
+
+@[simp] theorem iff_true : (a ↔ True) ↔ a := ⟨fun h => h.2 ⟨⟩, iff_true_intro⟩
+
+@[simp] theorem true_iff : (True ↔ a) ↔ a := iff_comm.trans iff_true
+
+@[simp] theorem iff_false : (a ↔ False) ↔ ¬a := ⟨Iff.mp, iff_false_intro⟩
+
+@[simp] theorem false_iff : (False ↔ a) ↔ ¬a := iff_comm.trans iff_false
+
+@[simp] theorem iff_self : (a ↔ a) ↔ True := iff_true_intro Iff.rfl
+
+theorem iff_congr (h₁ : a ↔ c) (h₂ : b ↔ d) : (a ↔ b) ↔ (c ↔ d) :=
+⟨fun h => h₁.symm.trans $ h.trans h₂, fun h => h₁.trans $ h.trans h₂.symm⟩
+
+@[simp] theorem imp_true_iff : (α → True) ↔ True := iff_true_intro fun _ => ⟨⟩
+
+@[simp] theorem false_imp_iff : (False → a) ↔ True := iff_true_intro False.elim
+
+def ExistsUnique (p : α → Prop) := ∃ x, p x ∧ ∀ y, p y → y = x
+
+open Lean in
+macro "∃! " xs:explicitBinders ", " b:term : term => expandExplicitBinders ``ExistsUnique xs b
+
+theorem ExistsUnique.intro {p : α → Prop} (w : α)
+  (h₁ : p w) (h₂ : ∀ y, p y → y = w) : ∃! x, p x := ⟨w, h₁, h₂⟩
+
+theorem ExistsUnique.exists {p : α → Prop} : (∃! x, p x) → ∃ x, p x | ⟨x, h, _⟩ => ⟨x, h⟩
+
+theorem ExistsUnique.unique {p : α → Prop} (h : ∃! x, p x)
+  {y₁ y₂ : α} (py₁ : p y₁) (py₂ : p y₂) : y₁ = y₂ :=
+let ⟨x, hx, hy⟩ := h; (hy _ py₁).trans (hy _ py₂).symm
+
+theorem forall_congr {p q : α → Prop} (h : ∀ a, p a ↔ q a) : (∀ a, p a) ↔ ∀ a, q a :=
+⟨fun H a => (h a).1 (H a), fun H a => (h a).2 (H a)⟩
+
+theorem Exists.imp {p q : α → Prop} (h : ∀ a, p a → q a) : (∃ a, p a) → ∃ a, q a
+| ⟨a, ha⟩ => ⟨a, h a ha⟩
+
+theorem exists_congr {p q : α → Prop} (h : ∀ a, p a ↔ q a) : (∃ a, p a) ↔ ∃ a, q a :=
+⟨Exists.imp fun x => (h x).1, Exists.imp fun x => (h x).2⟩
+
+theorem exists_unique_congr {p q : α → Prop} (h : ∀ a, p a ↔ q a) : (∃! a, p a) ↔ ∃! a, q a :=
+exists_congr fun x => and_congr (h _) $ forall_congr fun y => imp_congr_left (h _)
+
+theorem forall_not_of_not_exists {p : α → Prop} (hne : ¬∃ x, p x) (x) : ¬p x | hp => hne ⟨x, hp⟩
+
+instance forall_prop_decidable {p} (P : p → Prop)
+  [Dp : Decidable p] [DP : ∀ h, Decidable (P h)] : Decidable (∀ h, P h) :=
+  if h : p
+  then decidableOfDecidableOfIff (DP h) ⟨λ h2 _ => h2, λ al => al h⟩
+  else isTrue (λ h2 => absurd h2 h)
+
+@[simp] theorem forall_eq {p : α → Prop} {a' : α} : (∀a, a = a' → p a) ↔ p a' :=
+⟨λ h => h a' rfl, λ h a e => e.symm ▸ h⟩
+
+theorem forall_and_distrib {p q : α → Prop} : (∀ x, p x ∧ q x) ↔ (∀ x, p x) ∧ (∀ x, q x) :=
+⟨λ h => ⟨λ x => (h x).left, λ x => (h x).right⟩, λ ⟨h₁, h₂⟩ x => ⟨h₁ x, h₂ x⟩⟩
+
+def Decidable.by_cases := @byCases
+def Decidable.by_contradiction := @byContradiction
+def Decidable.of_not_not := @ofNotNot
+
+theorem Decidable.not_and [Decidable p] [Decidable q] : ¬ (p ∧ q) ↔ ¬ p ∨ ¬ q := notAndIffOrNot _ _
+
+@[inline] def Or.by_cases [Decidable p] (h : p ∨ q) (h₁ : p → α) (h₂ : q → α) : α :=
+if hp : p then h₁ hp else h₂ (h.resolve_left hp)
+
+@[inline] def Or.by_cases' [Decidable q] (h : p ∨ q) (h₁ : p → α) (h₂ : q → α) : α :=
+if hq : q then h₂ hq else h₁ (h.resolve_right hq)
+
+theorem Exists.nonempty {p : α → Prop} : (∃ x, p x) → Nonempty α | ⟨x, _⟩ => ⟨x⟩
+
+@[simp] def if_pos := @ifPos
+@[simp] def if_neg := @ifNeg
+@[simp] def dif_pos := @difPos
+@[simp] def dif_neg := @difNeg
+
+theorem ite_id [h : Decidable c] {α} (t : α) : (if c then t else t) = t := by cases h <;> rfl
+
+@[simp] theorem if_true {h : Decidable True} (t e : α) : (@ite α True h t e) = t :=
+if_pos trivial
+
+@[simp] theorem if_false {h : Decidable False} (t e : α) : (@ite α False h t e) = e :=
+if_neg not_false
+
+theorem dif_eq_if [h : Decidable c] {α} (t : α) (e : α) : (if h : c then t else e) = ite c t e :=
+by cases h <;> rfl
+
+/-- Universe lifting operation -/
+structure ulift.{r, s} (α : Type s) : Type (max s r) :=
+up :: (down : α)
+
+namespace ulift
+/- Bijection between α and ulift.{v} α -/
+theorem up_down {α : Type u} : ∀ (b : ulift.{v} α), up (down b) = b
+| up a => rfl
+
+theorem down_up {α : Type u} (a : α) : down (up.{v} a) = a := rfl
+end ulift
+
+/-- Universe lifting operation from Sort to Type -/
+structure plift (α : Sort u) : Type u :=
+up :: (down : α)
+
+namespace plift
+/- Bijection between α and plift α -/
+theorem up_down : ∀ (b : plift α), up (down b) = b
+| (up a) => rfl
+
+theorem down_up (a : α) : down (up a) = a := rfl
+end plift
+
+namespace WellFounded
+
+variable {α : Sort u} {C : α → Sort v} {r : α → α → Prop}
+
+unsafe def fix'.impl (hwf : WellFounded r) (F : ∀ x, (∀ y, r y x → C y) → C x) (x : α) : C x :=
+  F x fun y _ => impl hwf F y
+
+set_option codegen false in
+@[implementedBy fix'.impl]
+def fix' (hwf : WellFounded r) (F : ∀ x, (∀ y, r y x → C y) → C x) (x : α) : C x := hwf.fix F x
+
+end WellFounded
+
+-- Below are items ported from mathlib/src/logic/basic.lean
+
+theorem iff_of_eq (e : a = b) : a ↔ b := e ▸ Iff.rfl
+
+def decidable_of_iff (a : Prop) (h : a ↔ b) [D : Decidable a] : Decidable b :=
+decidableOfDecidableOfIff D h
+
+/-
+Stuff from mathlib's logic/basic.lean.
+TODO: import the whole thing.
+-/
+
+theorem or_imp_distrib : (a ∨ b → c) ↔ (a → c) ∧ (b → c) :=
+⟨fun h => ⟨fun ha => h (Or.inl ha), fun hb => h (Or.inr hb)⟩,
+  fun ⟨ha, hb⟩ => Or.rec ha hb⟩
+
+@[simp] theorem and_imp : (a ∧ b → c) ↔ (a → b → c) :=
+Iff.intro (λ h ha hb => h ⟨ha, hb⟩) (λ h ⟨ha, hb⟩ => h ha hb)
+
+@[simp] theorem not_and : ¬ (a ∧ b) ↔ (a → ¬ b) := and_imp
+
+@[simp] theorem exists_imp_distrib {p : α → Prop} : ((∃ x, p x) → b) ↔ ∀ x, p x → b :=
+⟨λ h x hpx => h ⟨x, hpx⟩, λ h ⟨x, hpx⟩ => h x hpx⟩
+
+@[simp] theorem exists_false : ¬ (∃a:α, False) := fun ⟨a, h⟩ => h
+
+@[simp] theorem exists_and_distrib_left {q : Prop} {p : α → Prop} :
+  (∃x, q ∧ p x) ↔ q ∧ (∃x, p x) :=
+⟨λ ⟨x, hq, hp⟩ => ⟨hq, x, hp⟩, λ ⟨hq, x, hp⟩ => ⟨x, hq, hp⟩⟩
+
+@[simp] theorem exists_and_distrib_right {q : Prop} {p : α → Prop} :
+  (∃x, p x ∧ q) ↔ (∃x, p x) ∧ q :=
+by simp [and_comm]
+
+@[simp] theorem exists_eq {a' : α} : ∃ a, a = a' := ⟨_, rfl⟩
+
+@[simp] theorem exists_eq' {a' : α} : ∃ a, a' = a := ⟨_, rfl⟩
+
+@[simp] theorem exists_eq_left {p : α → Prop} {a' : α} : (∃ a, a = a' ∧ p a) ↔ p a' :=
+⟨λ ⟨a, e, h⟩ => e ▸ h, λ h => ⟨_, rfl, h⟩⟩
+
+@[simp] theorem exists_eq_right {p : α → Prop} {a' : α} : (∃ a, p a ∧ a = a') ↔ p a' :=
+(exists_congr $ by exact λ a => and_comm).trans exists_eq_left
+
+@[simp] theorem exists_eq_left' {p : α → Prop} {a' : α} : (∃ a, a' = a ∧ p a) ↔ p a' :=
+by simp [@eq_comm _ a']
+
+protected theorem decidable.not_imp_symm [Decidable a] (h : ¬a → b) (hb : ¬b) : a :=
+Decidable.by_contradiction $ hb ∘ h
+
+theorem not.decidable_imp_symm [Decidable a] : (¬a → b) → ¬b → a := decidable.not_imp_symm
+
+theorem not_forall_of_exists_not {p : α → Prop} : (∃ x, ¬ p x) → ¬ ∀ x, p x
+| ⟨x, hn⟩, h => hn (h x)
+
+protected theorem Decidable.not_forall {p : α → Prop}
+  [Decidable (∃ x, ¬ p x)] [∀ x, Decidable (p x)] : (¬ ∀ x, p x) ↔ ∃ x, ¬ p x :=
+⟨not.decidable_imp_symm $ λ nx x => not.decidable_imp_symm (λ h => ⟨x, h⟩) nx,
+ not_forall_of_exists_not⟩
+
+@[simp] theorem not_exists {p : α → Prop} : (¬ ∃ x, p x) ↔ ∀ x, ¬ p x :=
+exists_imp_distrib
+
+open Classical
+
+@[simp] theorem not_forall {p : α → Prop} : (¬ ∀ x, p x) ↔ ∃ x, ¬ p x := Decidable.not_forall
