tests/TacticConfig.lean
@@ -1,0 +1,38 @@
+/-
+Copyright (c) 2021 Jannis Limperg. All rights reserved.
+Released under Apache 2.0 license as described in the file LICENSE.
+Authors: Jannis Limperg
+-/
+
+-- TODO clean up this test case
+
+import Aesop.Main
+
+inductive Even : Nat → Prop
+| zero : Even Nat.zero
+| plus_two {n} : Even n → Even (Nat.succ (Nat.succ n))
+
+inductive Odd : Nat → Prop
+| one : Odd (Nat.succ Nat.zero)
+| plus_two {n} : Odd n → Odd (Nat.succ (Nat.succ n))
+
+inductive EvenOrOdd : Nat → Prop
+| even {n} : Even n → EvenOrOdd n
+| odd {n} : Odd n → EvenOrOdd n
+
+set_option pp.all false
+sudo set_option trace.Aesop.RuleSet false
+sudo set_option trace.Aesop.Steps false
+
+-- We can add constants as rules.
+example : EvenOrOdd 3 := by
+  aesop
+    (safe [Even.zero, Even.plus_two, Odd.one, Odd.plus_two])
+    (unsafe [EvenOrOdd.even 50% (builder apply), EvenOrOdd.odd 50%])
+
+-- Same with local hypotheses, or a mix.
+example : EvenOrOdd 3 := by
+  have h₂ : ∀ n, Odd n → EvenOrOdd n := λ _ p => EvenOrOdd.odd p
+  aesop
+    (safe [Odd.one, Odd.plus_two])
+    (unsafe [EvenOrOdd.even 50%, h₂ 50%])
